wrote condition on divi node

project/out/Browser.ml
@@ -1,0 +1,956 @@
+open Prims
+type win_ref = Prims.nat
+let (fresh_win_ref : win_ref -> win_ref) = fun win -> win + Prims.int_one
+type page_ref = Prims.nat
+let (fresh_page_ref : page_ref -> page_ref) =
+  fun page -> page + Prims.int_one
+type node_ref = Prims.nat
+let (fresh_node_ref : node_ref -> node_ref) =
+  fun node -> node + Prims.int_one
+type act_ref = Prims.nat
+let (fresh_act_ref : act_ref -> act_ref) = fun act -> act + Prims.int_one
+type cookie_id =
+  {
+  cookie_id_domain: BrowserIO.domain ;
+  cookie_id_path: BrowserIO.path ;
+  cookie_id_key: Prims.string }
+let (__proj__Mkcookie_id__item__cookie_id_domain :
+  cookie_id -> BrowserIO.domain) =
+  fun projectee ->
+    match projectee with
+    | { cookie_id_domain; cookie_id_path; cookie_id_key;_} ->
+        cookie_id_domain
+let (__proj__Mkcookie_id__item__cookie_id_path : cookie_id -> BrowserIO.path)
+  =
+  fun projectee ->
+    match projectee with
+    | { cookie_id_domain; cookie_id_path; cookie_id_key;_} -> cookie_id_path
+let (__proj__Mkcookie_id__item__cookie_id_key : cookie_id -> Prims.string) =
+  fun projectee ->
+    match projectee with
+    | { cookie_id_domain; cookie_id_path; cookie_id_key;_} -> cookie_id_key
+type win_name =
+  | No_name 
+  | Str_name of Prims.string 
+let (uu___is_No_name : win_name -> Prims.bool) =
+  fun projectee -> match projectee with | No_name -> true | uu___ -> false
+let (uu___is_Str_name : win_name -> Prims.bool) =
+  fun projectee ->
+    match projectee with | Str_name _0 -> true | uu___ -> false
+let (__proj__Str_name__item___0 : win_name -> Prims.string) =
+  fun projectee -> match projectee with | Str_name _0 -> _0
+type win_opener =
+  | No_opener 
+  | Win_opener of win_ref 
+let (uu___is_No_opener : win_opener -> Prims.bool) =
+  fun projectee -> match projectee with | No_opener -> true | uu___ -> false
+let (uu___is_Win_opener : win_opener -> Prims.bool) =
+  fun projectee ->
+    match projectee with | Win_opener _0 -> true | uu___ -> false
+let (__proj__Win_opener__item___0 : win_opener -> win_ref) =
+  fun projectee -> match projectee with | Win_opener _0 -> _0
+type win = {
+  win_name: win_name ;
+  win_opener: win_opener ;
+  win_page: page_ref }
+let (__proj__Mkwin__item__win_name : win -> win_name) =
+  fun projectee ->
+    match projectee with
+    | { win_name = win_name1; win_opener = win_opener1; win_page;_} ->
+        win_name1
+let (__proj__Mkwin__item__win_opener : win -> win_opener) =
+  fun projectee ->
+    match projectee with
+    | { win_name = win_name1; win_opener = win_opener1; win_page;_} ->
+        win_opener1
+let (__proj__Mkwin__item__win_page : win -> page_ref) =
+  fun projectee ->
+    match projectee with
+    | { win_name = win_name1; win_opener = win_opener1; win_page;_} ->
+        win_page
+type context = {
+  context_win: win_ref ;
+  context_act: act_ref }
+let (__proj__Mkcontext__item__context_win : context -> win_ref) =
+  fun projectee ->
+    match projectee with | { context_win; context_act;_} -> context_win
+let (__proj__Mkcontext__item__context_act : context -> act_ref) =
+  fun projectee ->
+    match projectee with | { context_win; context_act;_} -> context_act
+type inner =
+  | Scoped_expr of (context * inner BrowserIO.expr) 
+  | R of value 
+and value =
+  | Closure of context * BrowserIO.var * BrowserIO.var Prims.list * inner
+  BrowserIO.expr 
+  | Win_value of win_ref 
+  | Node_value of node_ref 
+  | Null_value 
+  | Bool_value of Prims.bool 
+  | Int_value of Prims.int 
+  | String_value of Prims.string 
+  | Url_value of BrowserIO.url 
+  | Type_value of BrowserIO.typ 
+  | Code_value of unit BrowserIO.expr 
+  | Error of Prims.string 
+let (uu___is_Scoped_expr : inner -> Prims.bool) =
+  fun projectee ->
+    match projectee with | Scoped_expr _0 -> true | uu___ -> false
+let (__proj__Scoped_expr__item___0 :
+  inner -> (context * inner BrowserIO.expr)) =
+  fun projectee -> match projectee with | Scoped_expr _0 -> _0
+let (uu___is_R : inner -> Prims.bool) =
+  fun projectee -> match projectee with | R _0 -> true | uu___ -> false
+let (__proj__R__item___0 : inner -> value) =
+  fun projectee -> match projectee with | R _0 -> _0
+let (uu___is_Closure : value -> Prims.bool) =
+  fun projectee ->
+    match projectee with | Closure (_0, _1, _2, _3) -> true | uu___ -> false
+let (__proj__Closure__item___0 : value -> context) =
+  fun projectee -> match projectee with | Closure (_0, _1, _2, _3) -> _0
+let (__proj__Closure__item___1 : value -> BrowserIO.var) =
+  fun projectee -> match projectee with | Closure (_0, _1, _2, _3) -> _1
+let (__proj__Closure__item___2 : value -> BrowserIO.var Prims.list) =
+  fun projectee -> match projectee with | Closure (_0, _1, _2, _3) -> _2
+let (__proj__Closure__item___3 : value -> inner BrowserIO.expr) =
+  fun projectee -> match projectee with | Closure (_0, _1, _2, _3) -> _3
+let (uu___is_Win_value : value -> Prims.bool) =
+  fun projectee ->
+    match projectee with | Win_value _0 -> true | uu___ -> false
+let (__proj__Win_value__item___0 : value -> win_ref) =
+  fun projectee -> match projectee with | Win_value _0 -> _0
+let (uu___is_Node_value : value -> Prims.bool) =
+  fun projectee ->
+    match projectee with | Node_value _0 -> true | uu___ -> false
+let (__proj__Node_value__item___0 : value -> node_ref) =
+  fun projectee -> match projectee with | Node_value _0 -> _0
+let (uu___is_Null_value : value -> Prims.bool) =
+  fun projectee -> match projectee with | Null_value -> true | uu___ -> false
+let (uu___is_Bool_value : value -> Prims.bool) =
+  fun projectee ->
+    match projectee with | Bool_value _0 -> true | uu___ -> false
+let (__proj__Bool_value__item___0 : value -> Prims.bool) =
+  fun projectee -> match projectee with | Bool_value _0 -> _0
+let (uu___is_Int_value : value -> Prims.bool) =
+  fun projectee ->
+    match projectee with | Int_value _0 -> true | uu___ -> false
+let (__proj__Int_value__item___0 : value -> Prims.int) =
+  fun projectee -> match projectee with | Int_value _0 -> _0
+let (uu___is_String_value : value -> Prims.bool) =
+  fun projectee ->
+    match projectee with | String_value _0 -> true | uu___ -> false
+let (__proj__String_value__item___0 : value -> Prims.string) =
+  fun projectee -> match projectee with | String_value _0 -> _0
+let (uu___is_Url_value : value -> Prims.bool) =
+  fun projectee ->
+    match projectee with | Url_value _0 -> true | uu___ -> false
+let (__proj__Url_value__item___0 : value -> BrowserIO.url) =
+  fun projectee -> match projectee with | Url_value _0 -> _0
+let (uu___is_Type_value : value -> Prims.bool) =
+  fun projectee ->
+    match projectee with | Type_value _0 -> true | uu___ -> false
+let (__proj__Type_value__item___0 : value -> BrowserIO.typ) =
+  fun projectee -> match projectee with | Type_value _0 -> _0
+let (uu___is_Code_value : value -> Prims.bool) =
+  fun projectee ->
+    match projectee with | Code_value _0 -> true | uu___ -> false
+let (__proj__Code_value__item___0 : value -> Prims.l_False BrowserIO.expr) =
+  fun projectee -> match projectee with | Code_value _0 -> _0
+let (uu___is_Error : value -> Prims.bool) =
+  fun projectee -> match projectee with | Error _0 -> true | uu___ -> false
+let (__proj__Error__item___0 : value -> Prims.string) =
+  fun projectee -> match projectee with | Error _0 -> _0
+let (prim1 : Prims.string -> value -> value) =
+  fun prim ->
+    fun r ->
+      match (prim, r) with
+      | ("!", Bool_value bl) -> Bool_value (Prims.op_Negation bl)
+      | ("-", Int_value n) -> Int_value (- n)
+      | ("typeof", Null_value) -> Type_value BrowserIO.Null_type
+      | ("typeof", Bool_value uu___) -> Type_value BrowserIO.Bool_type
+      | ("typeof", Int_value uu___) -> Type_value BrowserIO.Int_type
+      | ("typeof", String_value uu___) -> Type_value BrowserIO.String_type
+      | ("typeof", Url_value uu___) -> Type_value BrowserIO.Url_type
+      | ("typeof", Type_value uu___) -> Type_value BrowserIO.Type_type
+      | ("typeof", Code_value uu___) -> Type_value BrowserIO.Code_type
+      | ("typeof", Win_value uu___) -> Type_value BrowserIO.Window_type
+      | ("typeof", Node_value uu___) -> Type_value BrowserIO.Node_type
+      | ("typeof", Closure (uu___, uu___1, uu___2, uu___3)) ->
+          Type_value BrowserIO.Function_type
+      | ("StringToInt", String_value s) ->
+          Int_value (Assumed.int_of_string s)
+      | ("IntToString", Int_value i) -> String_value (Prims.string_of_int i)
+      | (uu___, Error uu___1) -> r
+      | (uu___, uu___1) ->
+          Error
+            (Prims.strcat "primitive operation ("
+               (Prims.strcat prim ") is not implemented on this type"))
+let (prim2 : Prims.string -> value -> value -> value) =
+  fun prim ->
+    fun r1 ->
+      fun r2 ->
+        match (prim, r1, r2) with
+        | ("==", uu___, uu___1) -> Bool_value (r1 = r2)
+        | ("||", Bool_value bl1, Bool_value bl2) -> Bool_value (bl1 || bl2)
+        | ("&&", Bool_value bl1, Bool_value bl2) -> Bool_value (bl1 && bl2)
+        | ("+", String_value s1, String_value s2) ->
+            String_value (Prims.strcat s1 s2)
+        | ("*", Int_value n1, Int_value n2) -> Int_value (n1 * n2)
+        | ("+", Int_value n1, Int_value n2) -> Int_value (n1 + n2)
+        | ("-", Int_value n1, Int_value n2) -> Int_value (n1 - n2)
+        | ("addtourl", Url_value u, String_value s) ->
+            Url_value
+              ((match u with
+                | BrowserIO.Blank_url -> BrowserIO.Blank_url
+                | BrowserIO.Http_url
+                    (domain,
+                     { BrowserIO.req_uri_path = path;
+                       BrowserIO.req_uri_params = params;_})
+                    ->
+                    BrowserIO.Http_url
+                      (domain,
+                        {
+                          BrowserIO.req_uri_path = path;
+                          BrowserIO.req_uri_params =
+                            (Prims.strcat params (Prims.strcat "?t=" s))
+                        })))
+        | (uu___, Error uu___1, uu___2) -> r1
+        | (uu___, uu___1, Error uu___2) -> r2
+        | (uu___, uu___1, uu___2) ->
+            Error
+              (Prims.strcat "primitive operation ("
+                 (Prims.strcat prim ") is not implemented for these types"))
+let rec (to_inner_expr : unit BrowserIO.expr -> inner BrowserIO.expr) =
+  fun e ->
+    let f = to_inner_expr in
+    match e with
+    | BrowserIO.X uu___ -> BrowserIO.Null
+    | BrowserIO.Null -> BrowserIO.Null
+    | BrowserIO.Bool b -> BrowserIO.Bool b
+    | BrowserIO.Int n -> BrowserIO.Int n
+    | BrowserIO.String s -> BrowserIO.String s
+    | BrowserIO.Url u -> BrowserIO.Url u
+    | BrowserIO.Types t -> BrowserIO.Types t
+    | BrowserIO.Code e1 -> BrowserIO.Code e1
+    | BrowserIO.Eval e1 -> BrowserIO.Eval (f e1)
+    | BrowserIO.Var x -> BrowserIO.Var x
+    | BrowserIO.Function (x, xs, e1) -> BrowserIO.Function (x, xs, (f e1))
+    | BrowserIO.Apply (e1, e2) -> BrowserIO.Apply ((f e1), (f e2))
+    | BrowserIO.Prim1 (s, e1) -> BrowserIO.Prim1 (s, (f e1))
+    | BrowserIO.Prim2 (s, e1, e2) -> BrowserIO.Prim2 (s, (f e1), (f e2))
+    | BrowserIO.Alert e1 -> BrowserIO.Alert (f e1)
+    | BrowserIO.If (e1, e2, e3) -> BrowserIO.If ((f e1), (f e2), (f e3))
+    | BrowserIO.While (e1, e2) -> BrowserIO.While ((f e1), (f e2))
+    | BrowserIO.Set_var (var, e1) -> BrowserIO.Set_var (var, (f e1))
+    | BrowserIO.Seq (e1, e2) -> BrowserIO.Seq ((f e1), (f e2))
+    | BrowserIO.Get_cookie (e1, e2) -> BrowserIO.Get_cookie ((f e1), (f e2))
+    | BrowserIO.Set_cookie (e1, e2, e3) ->
+        BrowserIO.Set_cookie ((f e1), (f e2), (f e3))
+    | BrowserIO.Xhr (e1, e2, e3) -> BrowserIO.Xhr ((f e1), (f e2), (f e3))
+    | BrowserIO.Self_win -> BrowserIO.Self_win
+    | BrowserIO.Named_win e1 -> BrowserIO.Named_win (f e1)
+    | BrowserIO.Open_win e1 -> BrowserIO.Open_win (f e1)
+    | BrowserIO.Open_named_win (e1, e2) ->
+        BrowserIO.Open_named_win ((f e1), (f e2))
+    | BrowserIO.Close_win e1 -> BrowserIO.Close_win (f e1)
+    | BrowserIO.Navigate_win (e1, e2) ->
+        BrowserIO.Navigate_win ((f e1), (f e2))
+    | BrowserIO.Is_win_closed e1 -> BrowserIO.Is_win_closed (f e1)
+    | BrowserIO.Get_win_opener e1 -> BrowserIO.Get_win_opener (f e1)
+    | BrowserIO.Get_win_location e1 -> BrowserIO.Get_win_location (f e1)
+    | BrowserIO.Get_win_name e1 -> BrowserIO.Get_win_name (f e1)
+    | BrowserIO.Set_win_name (e1, e2) ->
+        BrowserIO.Set_win_name ((f e1), (f e2))
+    | BrowserIO.Get_win_root_node e1 -> BrowserIO.Get_win_root_node (f e1)
+    | BrowserIO.Set_win_root_node (e1, e2) ->
+        BrowserIO.Set_win_root_node ((f e1), (f e2))
+    | BrowserIO.Get_win_var (e1, var) -> BrowserIO.Get_win_var ((f e1), var)
+    | BrowserIO.Set_win_var (e1, var, e2) ->
+        BrowserIO.Set_win_var ((f e1), var, (f e2))
+    | BrowserIO.New_node e1 -> BrowserIO.New_node (f e1)
+    | BrowserIO.Get_node_type e1 -> BrowserIO.Get_node_type (f e1)
+    | BrowserIO.Get_node_contents e1 -> BrowserIO.Get_node_contents (f e1)
+    | BrowserIO.Set_node_contents (e1, e2) ->
+        BrowserIO.Set_node_contents ((f e1), (f e2))
+    | BrowserIO.Get_node_attr (e1, e2) ->
+        BrowserIO.Get_node_attr ((f e1), (f e2))
+    | BrowserIO.Set_node_attr (e1, e2, e3) ->
+        BrowserIO.Set_node_attr ((f e1), (f e2), (f e3))
+    | BrowserIO.Remove_handlers e1 -> BrowserIO.Remove_handlers (f e1)
+    | BrowserIO.Add_handler (e1, e2) ->
+        BrowserIO.Add_handler ((f e1), (f e2))
+    | BrowserIO.Get_parent e1 -> BrowserIO.Get_parent (f e1)
+    | BrowserIO.Get_child (e1, e2) -> BrowserIO.Get_child ((f e1), (f e2))
+    | BrowserIO.Insert_node (e1, e2, e3) ->
+        BrowserIO.Insert_node ((f e1), (f e2), (f e3))
+    | BrowserIO.Remove_node e1 -> BrowserIO.Remove_node (f e1)
+type node =
+  | Para_node of (BrowserIO.elt_id FStar_Pervasives_Native.option *
+  Prims.string) 
+  | Link_node of (BrowserIO.elt_id FStar_Pervasives_Native.option *
+  BrowserIO.url * Prims.string) 
+  | Textbox_node of (BrowserIO.elt_id FStar_Pervasives_Native.option *
+  Prims.string * value Prims.list) 
+  | Button_node of (BrowserIO.elt_id FStar_Pervasives_Native.option *
+  Prims.string * value Prims.list) 
+  | Inl_script_node of (BrowserIO.elt_id FStar_Pervasives_Native.option *
+  unit BrowserIO.expr * Prims.bool) 
+  | Rem_script_node of (BrowserIO.elt_id FStar_Pervasives_Native.option *
+  BrowserIO.url * Prims.bool) 
+  | Div_node of (BrowserIO.elt_id FStar_Pervasives_Native.option * node_ref
+  Prims.list) 
+let (uu___is_Para_node : node -> Prims.bool) =
+  fun projectee ->
+    match projectee with | Para_node _0 -> true | uu___ -> false
+let (__proj__Para_node__item___0 :
+  node -> (BrowserIO.elt_id FStar_Pervasives_Native.option * Prims.string)) =
+  fun projectee -> match projectee with | Para_node _0 -> _0
+let (uu___is_Link_node : node -> Prims.bool) =
+  fun projectee ->
+    match projectee with | Link_node _0 -> true | uu___ -> false
+let (__proj__Link_node__item___0 :
+  node ->
+    (BrowserIO.elt_id FStar_Pervasives_Native.option * BrowserIO.url *
+      Prims.string))
+  = fun projectee -> match projectee with | Link_node _0 -> _0
+let (uu___is_Textbox_node : node -> Prims.bool) =
+  fun projectee ->
+    match projectee with | Textbox_node _0 -> true | uu___ -> false
+let (__proj__Textbox_node__item___0 :
+  node ->
+    (BrowserIO.elt_id FStar_Pervasives_Native.option * Prims.string * value
+      Prims.list))
+  = fun projectee -> match projectee with | Textbox_node _0 -> _0
+let (uu___is_Button_node : node -> Prims.bool) =
+  fun projectee ->
+    match projectee with | Button_node _0 -> true | uu___ -> false
+let (__proj__Button_node__item___0 :
+  node ->
+    (BrowserIO.elt_id FStar_Pervasives_Native.option * Prims.string * value
+      Prims.list))
+  = fun projectee -> match projectee with | Button_node _0 -> _0
+let (uu___is_Inl_script_node : node -> Prims.bool) =
+  fun projectee ->
+    match projectee with | Inl_script_node _0 -> true | uu___ -> false
+let (__proj__Inl_script_node__item___0 :
+  node ->
+    (BrowserIO.elt_id FStar_Pervasives_Native.option * unit BrowserIO.expr *
+      Prims.bool))
+  = fun projectee -> match projectee with | Inl_script_node _0 -> _0
+let (uu___is_Rem_script_node : node -> Prims.bool) =
+  fun projectee ->
+    match projectee with | Rem_script_node _0 -> true | uu___ -> false
+let (__proj__Rem_script_node__item___0 :
+  node ->
+    (BrowserIO.elt_id FStar_Pervasives_Native.option * BrowserIO.url *
+      Prims.bool))
+  = fun projectee -> match projectee with | Rem_script_node _0 -> _0
+let (uu___is_Div_node : node -> Prims.bool) =
+  fun projectee ->
+    match projectee with | Div_node _0 -> true | uu___ -> false
+let (__proj__Div_node__item___0 :
+  node ->
+    (BrowserIO.elt_id FStar_Pervasives_Native.option * node_ref Prims.list))
+  = fun projectee -> match projectee with | Div_node _0 -> _0
+type queued_expr =
+  | Known_expr of inner BrowserIO.expr 
+  | Unknown_expr of node_ref 
+let (uu___is_Known_expr : queued_expr -> Prims.bool) =
+  fun projectee ->
+    match projectee with | Known_expr _0 -> true | uu___ -> false
+let (__proj__Known_expr__item___0 : queued_expr -> inner BrowserIO.expr) =
+  fun projectee -> match projectee with | Known_expr _0 -> _0
+let (uu___is_Unknown_expr : queued_expr -> Prims.bool) =
+  fun projectee ->
+    match projectee with | Unknown_expr _0 -> true | uu___ -> false
+let (__proj__Unknown_expr__item___0 : queued_expr -> node_ref) =
+  fun projectee -> match projectee with | Unknown_expr _0 -> _0
+type page =
+  {
+  page_location: BrowserIO.url ;
+  page_document: node_ref FStar_Pervasives_Native.option ;
+  page_environment: act_ref ;
+  page_script_queue: queued_expr Prims.list }
+let (__proj__Mkpage__item__page_location : page -> BrowserIO.url) =
+  fun projectee ->
+    match projectee with
+    | { page_location; page_document; page_environment; page_script_queue;_}
+        -> page_location
+let (__proj__Mkpage__item__page_document :
+  page -> node_ref FStar_Pervasives_Native.option) =
+  fun projectee ->
+    match projectee with
+    | { page_location; page_document; page_environment; page_script_queue;_}
+        -> page_document
+let (__proj__Mkpage__item__page_environment : page -> act_ref) =
+  fun projectee ->
+    match projectee with
+    | { page_location; page_document; page_environment; page_script_queue;_}
+        -> page_environment
+let (__proj__Mkpage__item__page_script_queue :
+  page -> queued_expr Prims.list) =
+  fun projectee ->
+    match projectee with
+    | { page_location; page_document; page_environment; page_script_queue;_}
+        -> page_script_queue
+type act =
+  {
+  act_parent: act_ref FStar_Pervasives_Native.option ;
+  act_vars: (BrowserIO.var * value) Prims.list }
+let (__proj__Mkact__item__act_parent :
+  act -> act_ref FStar_Pervasives_Native.option) =
+  fun projectee ->
+    match projectee with | { act_parent; act_vars;_} -> act_parent
+let (__proj__Mkact__item__act_vars :
+  act -> (BrowserIO.var * value) Prims.list) =
+  fun projectee ->
+    match projectee with | { act_parent; act_vars;_} -> act_vars
+type dst =
+  | Xhr_dst of (page_ref * value) 
+  | Doc_dst of win_ref 
+  | Script_dst of (page_ref * node_ref) 
+let (uu___is_Xhr_dst : dst -> Prims.bool) =
+  fun projectee -> match projectee with | Xhr_dst _0 -> true | uu___ -> false
+let (__proj__Xhr_dst__item___0 : dst -> (page_ref * value)) =
+  fun projectee -> match projectee with | Xhr_dst _0 -> _0
+let (uu___is_Doc_dst : dst -> Prims.bool) =
+  fun projectee -> match projectee with | Doc_dst _0 -> true | uu___ -> false
+let (__proj__Doc_dst__item___0 : dst -> win_ref) =
+  fun projectee -> match projectee with | Doc_dst _0 -> _0
+let (uu___is_Script_dst : dst -> Prims.bool) =
+  fun projectee ->
+    match projectee with | Script_dst _0 -> true | uu___ -> false
+let (__proj__Script_dst__item___0 : dst -> (page_ref * node_ref)) =
+  fun projectee -> match projectee with | Script_dst _0 -> _0
+type task = {
+  task_win: win_ref ;
+  task_expr: inner BrowserIO.expr }
+let (__proj__Mktask__item__task_win : task -> win_ref) =
+  fun projectee ->
+    match projectee with | { task_win; task_expr;_} -> task_win
+let (__proj__Mktask__item__task_expr : task -> inner BrowserIO.expr) =
+  fun projectee ->
+    match projectee with | { task_win; task_expr;_} -> task_expr
+let (b_act_ref_pred : act_ref -> act -> Prims.bool) =
+  fun r ->
+    fun a ->
+      match a.act_parent with
+      | FStar_Pervasives_Native.None -> true
+      | FStar_Pervasives_Native.Some ap -> r > ap
+let rec (b_env_pred : (act_ref * act) Prims.list -> Prims.bool) =
+  fun l ->
+    match l with
+    | [] -> true
+    | (r, a)::tl -> (b_act_ref_pred r a) && (b_env_pred tl)
+type b_env = (act_ref * act) Prims.list
+type browser =
+  {
+  browser_windows: (win_ref * win) Prims.list ;
+  browser_pages: (page_ref * page) Prims.list ;
+  browser_nodes: (node_ref * node) Prims.list ;
+  browser_environments: b_env ;
+  browser_cookies: (cookie_id * Prims.string) Prims.list ;
+  browser_connections:
+    (BrowserIO.domain * BrowserIO.req_uri * dst) Prims.list }
+let (__proj__Mkbrowser__item__browser_windows :
+  browser -> (win_ref * win) Prims.list) =
+  fun projectee ->
+    match projectee with
+    | { browser_windows; browser_pages; browser_nodes; browser_environments;
+        browser_cookies; browser_connections;_} -> browser_windows
+let (__proj__Mkbrowser__item__browser_pages :
+  browser -> (page_ref * page) Prims.list) =
+  fun projectee ->
+    match projectee with
+    | { browser_windows; browser_pages; browser_nodes; browser_environments;
+        browser_cookies; browser_connections;_} -> browser_pages
+let (__proj__Mkbrowser__item__browser_nodes :
+  browser -> (node_ref * node) Prims.list) =
+  fun projectee ->
+    match projectee with
+    | { browser_windows; browser_pages; browser_nodes; browser_environments;
+        browser_cookies; browser_connections;_} -> browser_nodes
+let (__proj__Mkbrowser__item__browser_environments : browser -> b_env) =
+  fun projectee ->
+    match projectee with
+    | { browser_windows; browser_pages; browser_nodes; browser_environments;
+        browser_cookies; browser_connections;_} -> browser_environments
+let (__proj__Mkbrowser__item__browser_cookies :
+  browser -> (cookie_id * Prims.string) Prims.list) =
+  fun projectee ->
+    match projectee with
+    | { browser_windows; browser_pages; browser_nodes; browser_environments;
+        browser_cookies; browser_connections;_} -> browser_cookies
+let (__proj__Mkbrowser__item__browser_connections :
+  browser -> (BrowserIO.domain * BrowserIO.req_uri * dst) Prims.list) =
+  fun projectee ->
+    match projectee with
+    | { browser_windows; browser_pages; browser_nodes; browser_environments;
+        browser_cookies; browser_connections;_} -> browser_connections
+let rec upd_assoc :
+  'key 'data .
+    'key -> 'data -> ('key * 'data) Prims.list -> ('key * 'data) Prims.list
+  =
+  fun k ->
+    fun d ->
+      fun map ->
+        match map with
+        | [] -> [(k, d)]
+        | (k', d')::map1 ->
+            if k' = k
+            then (k', d) :: map1
+            else (k', d') :: (upd_assoc k d map1)
+let rec find_pos :
+  'key 'data . 'key -> ('key * 'data) Prims.list -> Prims.int =
+  fun k ->
+    fun map ->
+      match map with
+      | [] -> Prims.int_zero
+      | (k', uu___)::map1 ->
+          if k' = k
+          then Prims.int_zero
+          else Prims.int_one + (find_pos k map1)
+let rec remove_assoc :
+  'key 'data . 'key -> ('key * 'data) Prims.list -> ('key * 'data) Prims.list
+  =
+  fun k ->
+    fun map ->
+      match map with
+      | [] -> []
+      | (k', d')::map1 ->
+          if k' = k then map1 else (k', d') :: (remove_assoc k map1)
+let (page_valid : page_ref -> browser -> Prims.bool) =
+  fun pr ->
+    fun b ->
+      match FStar_List_Tot_Base.assoc pr b.browser_pages with
+      | FStar_Pervasives_Native.None -> false
+      | uu___ -> true
+let (page_assoc : page_ref -> browser -> page FStar_Pervasives_Native.option)
+  = fun pr -> fun b -> FStar_List_Tot_Base.assoc pr b.browser_pages
+let (page_assoc_valid : page_ref -> browser -> page) =
+  fun pr ->
+    fun b ->
+      FStar_Pervasives_Native.__proj__Some__item__v
+        (FStar_List_Tot_Base.assoc pr b.browser_pages)
+let (page_update : page_ref -> page -> browser -> browser) =
+  fun pr ->
+    fun p ->
+      fun b ->
+        let pages' = upd_assoc pr p b.browser_pages in
+        {
+          browser_windows = (b.browser_windows);
+          browser_pages = pages';
+          browser_nodes = (b.browser_nodes);
+          browser_environments = (b.browser_environments);
+          browser_cookies = (b.browser_cookies);
+          browser_connections = (b.browser_connections)
+        }
+let (page_new : page -> browser -> (page_ref * browser)) =
+  fun p ->
+    fun b ->
+      let p_ref =
+        if (FStar_List_Tot_Base.length b.browser_pages) >= Prims.int_one
+        then
+          FStar_Pervasives_Native.fst
+            (FStar_List_Tot_Base.last b.browser_pages)
+        else Prims.int_zero in
+      let pr = fresh_page_ref p_ref in
+      let pages' = upd_assoc pr p b.browser_pages in
+      let b' =
+        {
+          browser_windows = (b.browser_windows);
+          browser_pages = pages';
+          browser_nodes = (b.browser_nodes);
+          browser_environments = (b.browser_environments);
+          browser_cookies = (b.browser_cookies);
+          browser_connections = (b.browser_connections)
+        } in
+      (pr, b')
+let (page_remove : page_ref -> browser -> browser) =
+  fun pr ->
+    fun b ->
+      let pages' = remove_assoc pr b.browser_pages in
+      {
+        browser_windows = (b.browser_windows);
+        browser_pages = pages';
+        browser_nodes = (b.browser_nodes);
+        browser_environments = (b.browser_environments);
+        browser_cookies = (b.browser_cookies);
+        browser_connections = (b.browser_connections)
+      }
+let (page_win :
+  page_ref -> browser -> win_ref FStar_Pervasives_Native.option) =
+  fun pr ->
+    fun b ->
+      let has_pr uu___ = match uu___ with | (uu___1, w) -> w.win_page = pr in
+      match FStar_List_Tot_Base.filter has_pr b.browser_windows with
+      | (wr, uu___)::[] -> FStar_Pervasives_Native.Some wr
+      | uu___ -> FStar_Pervasives_Native.None
+let (win_valid : win_ref -> browser -> Prims.bool) =
+  fun wr ->
+    fun b ->
+      match FStar_List_Tot_Base.assoc wr b.browser_windows with
+      | FStar_Pervasives_Native.None -> false
+      | uu___ -> true
+let (win_assoc : win_ref -> browser -> win FStar_Pervasives_Native.option) =
+  fun wr -> fun b -> FStar_List_Tot_Base.assoc wr b.browser_windows
+let (win_assoc_valid : win_ref -> browser -> win) =
+  fun wr ->
+    fun b ->
+      FStar_Pervasives_Native.__proj__Some__item__v
+        (FStar_List_Tot_Base.assoc wr b.browser_windows)
+let (win_update : win_ref -> win -> browser -> browser) =
+  fun wr ->
+    fun w ->
+      fun b ->
+        let windows' = upd_assoc wr w b.browser_windows in
+        {
+          browser_windows = windows';
+          browser_pages = (b.browser_pages);
+          browser_nodes = (b.browser_nodes);
+          browser_environments = (b.browser_environments);
+          browser_cookies = (b.browser_cookies);
+          browser_connections = (b.browser_connections)
+        }
+let (win_new : win -> browser -> (win_ref * browser)) =
+  fun w ->
+    fun b ->
+      let w_ref =
+        if (FStar_List_Tot_Base.length b.browser_windows) >= Prims.int_one
+        then
+          FStar_Pervasives_Native.fst
+            (FStar_List_Tot_Base.last b.browser_windows)
+        else Prims.int_zero in
+      let wr = fresh_win_ref w_ref in let b' = win_update wr w b in (wr, b')
+let (win_remove : win_ref -> browser -> browser) =
+  fun wr ->
+    fun b ->
+      match win_assoc wr b with
+      | FStar_Pervasives_Native.None -> b
+      | FStar_Pervasives_Native.Some w ->
+          let b' = page_remove w.win_page b in
+          let windows' = remove_assoc wr b'.browser_windows in
+          {
+            browser_windows = windows';
+            browser_pages = (b'.browser_pages);
+            browser_nodes = (b'.browser_nodes);
+            browser_environments = (b'.browser_environments);
+            browser_cookies = (b'.browser_cookies);
+            browser_connections = (b'.browser_connections)
+          }
+let (win_from_win_name :
+  Prims.string -> browser -> win_ref FStar_Pervasives_Native.option) =
+  fun str ->
+    fun b ->
+      let has_name uu___ =
+        match uu___ with | (uu___1, w) -> w.win_name = (Str_name str) in
+      match FStar_List_Tot_Base.filter has_name b.browser_windows with
+      | [] -> FStar_Pervasives_Native.None
+      | (wr, uu___)::uu___1 -> FStar_Pervasives_Native.Some wr
+let (win_from_user_window :
+  BrowserIO.user_window ->
+    BrowserIO.user_window ->
+      browser -> win_ref FStar_Pervasives_Native.option)
+  =
+  fun u ->
+    fun n -> fun b -> failwith "Not yet implemented:win_from_user_window"
+let (node_valid : node_ref -> browser -> Prims.bool) =
+  fun dr ->
+    fun b ->
+      match FStar_List_Tot_Base.assoc dr b.browser_windows with
+      | FStar_Pervasives_Native.None -> false
+      | uu___ -> true
+let (node_assoc_valid : node_ref -> browser -> node) =
+  fun dr ->
+    fun b ->
+      FStar_Pervasives_Native.__proj__Some__item__v
+        (FStar_List_Tot_Base.assoc dr b.browser_nodes)
+let (node_update : node_ref -> node -> browser -> browser) =
+  fun dr ->
+    fun dn ->
+      fun b ->
+        let nodes' = upd_assoc dr dn b.browser_nodes in
+        {
+          browser_windows = (b.browser_windows);
+          browser_pages = (b.browser_pages);
+          browser_nodes = nodes';
+          browser_environments = (b.browser_environments);
+          browser_cookies = (b.browser_cookies);
+          browser_connections = (b.browser_connections)
+        }
+let (node_new : node -> browser -> (node_ref * browser)) =
+  fun dn ->
+    fun b ->
+      let n_ref =
+        if (FStar_List_Tot_Base.length b.browser_nodes) >= Prims.int_one
+        then
+          FStar_Pervasives_Native.fst
+            (FStar_List_Tot_Base.last b.browser_nodes)
+        else Prims.int_zero in
+      let nr = fresh_win_ref n_ref in
+      let b' = node_update nr dn b in (nr, b')
+type node_parent_type =
+  | No_parent 
+  | Page_parent of page_ref 
+  | Parent_node of node_ref 
+let (uu___is_No_parent : node_parent_type -> Prims.bool) =
+  fun projectee -> match projectee with | No_parent -> true | uu___ -> false
+let (uu___is_Page_parent : node_parent_type -> Prims.bool) =
+  fun projectee ->
+    match projectee with | Page_parent _0 -> true | uu___ -> false
+let (__proj__Page_parent__item___0 : node_parent_type -> page_ref) =
+  fun projectee -> match projectee with | Page_parent _0 -> _0
+let (uu___is_Parent_node : node_parent_type -> Prims.bool) =
+  fun projectee ->
+    match projectee with | Parent_node _0 -> true | uu___ -> false
+let (__proj__Parent_node__item___0 : node_parent_type -> node_ref) =
+  fun projectee -> match projectee with | Parent_node _0 -> _0
+let (node_parent : node_ref -> browser -> node_parent_type) =
+  fun dr ->
+    fun b ->
+      let is_page_parent uu___ =
+        match uu___ with
+        | (uu___1, p) ->
+            (match p.page_document with
+             | FStar_Pervasives_Native.Some dr1 ->
+                 if dr1 = dr then true else false
+             | uu___2 -> false) in
+      let is_node_parent uu___ =
+        match uu___ with
+        | (uu___1, dn) ->
+            (match dn with
+             | Div_node (uu___2, children) ->
+                 FStar_List_Tot_Base.mem dr children
+             | uu___2 -> false) in
+      match FStar_List_Tot_Base.filter is_page_parent b.browser_pages with
+      | (pr, uu___)::uu___1 -> Page_parent pr
+      | [] ->
+          (match FStar_List_Tot_Base.filter is_node_parent b.browser_nodes
+           with
+           | (dr1, uu___)::uu___1 -> Parent_node dr1
+           | [] -> No_parent)
+let (node_page :
+  node_ref -> browser -> page_ref FStar_Pervasives_Native.option) =
+  fun dr -> fun b -> failwith "Not yet implemented:node_page"
+let (act_valid : act_ref -> browser -> Prims.bool) =
+  fun ar ->
+    fun b ->
+      match FStar_List_Tot_Base.assoc ar b.browser_environments with
+      | FStar_Pervasives_Native.None -> false
+      | uu___ -> true
+
+let (act_assoc_valid : act_ref -> browser -> act) =
+  fun ar ->
+    fun b ->
+      match FStar_List_Tot_Base.assoc ar b.browser_environments with
+      | FStar_Pervasives_Native.Some v -> v
+
+let (act_update : act_ref -> act -> browser -> browser) =
+  fun ar ->
+    fun act1 ->
+      fun b ->
+        let environments' = upd_assoc ar act1 b.browser_environments in
+        {
+          browser_windows = (b.browser_windows);
+          browser_pages = (b.browser_pages);
+          browser_nodes = (b.browser_nodes);
+          browser_environments = environments';
+          browser_cookies = (b.browser_cookies);
+          browser_connections = (b.browser_connections)
+        }
+let (act_new : act -> browser -> (act_ref * browser)) =
+  fun act1 ->
+    fun b ->
+      let a_ref =
+        if
+          (FStar_List_Tot_Base.length b.browser_environments) >=
+            Prims.int_one
+        then
+          FStar_Pervasives_Native.fst
+            (FStar_List_Tot_Base.last b.browser_environments)
+        else Prims.int_zero in
+      let ar = fresh_page_ref a_ref in
+      let b' = act_update ar act1 b in (ar, b')
+let rec (get_var :
+  BrowserIO.var -> act_ref -> browser -> value FStar_Pervasives_Native.option)
+  =
+  fun x ->
+    fun ar ->
+      fun b ->
+        if act_valid ar b
+        then
+          let act1 = act_assoc_valid ar b in
+          match FStar_List_Tot_Base.assoc x act1.act_vars with
+          | FStar_Pervasives_Native.None ->
+              (match act1.act_parent with
+               | FStar_Pervasives_Native.None -> FStar_Pervasives_Native.None
+               | FStar_Pervasives_Native.Some ar1 -> get_var x ar1 b)
+          | uu___ -> FStar_List_Tot_Base.assoc x act1.act_vars
+        else FStar_Pervasives_Native.None
+let (create_var :
+  BrowserIO.var ->
+    value -> act_ref -> browser -> browser FStar_Pervasives_Native.option)
+  =
+  fun x ->
+    fun r ->
+      fun ar ->
+        fun b ->
+          if act_valid ar b
+          then
+            let act1 = act_assoc_valid ar b in
+            let data' = upd_assoc x r act1.act_vars in
+            let act' = { act_parent = (act1.act_parent); act_vars = data' } in
+            FStar_Pervasives_Native.Some (act_update ar act' b)
+          else FStar_Pervasives_Native.None
+let rec (set_var :
+  BrowserIO.var ->
+    value -> act_ref -> browser -> browser FStar_Pervasives_Native.option)
+  =
+  fun x ->
+    fun r ->
+      fun ar ->
+        fun b ->
+          if act_valid ar b
+          then
+            let act1 = act_assoc_valid ar b in
+            match FStar_List_Tot_Base.assoc x act1.act_vars with
+            | FStar_Pervasives_Native.None ->
+                (match act1.act_parent with
+                 | FStar_Pervasives_Native.None -> create_var x r ar b
+                 | FStar_Pervasives_Native.Some ar1 -> set_var x r ar1 b)
+            | uu___ ->
+                let data' = upd_assoc x r act1.act_vars in
+                let act' =
+                  { act_parent = (act1.act_parent); act_vars = data' } in
+                FStar_Pervasives_Native.Some (act_update ar act' b)
+          else FStar_Pervasives_Native.None
+let rec prefix : 'a . 'a Prims.list -> 'a Prims.list -> Prims.bool =
+  fun xs ->
+    fun ys ->
+      match (xs, ys) with
+      | ([], uu___) -> true
+      | (x::xs', y::ys') -> (x = y) && (prefix xs' ys')
+      | (uu___, uu___1) -> false
+let (get_site_cookies :
+  BrowserIO.domain ->
+    BrowserIO.path -> browser -> (Prims.string * Prims.string) Prims.list)
+  =
+  fun d ->
+    fun p ->
+      fun b ->
+        let check uu___ =
+          match uu___ with
+          | (cid, uu___1) ->
+              ((cid.cookie_id_domain = d) && (prefix cid.cookie_id_path p))
+                ||
+                ((prefix cid.cookie_id_domain d) && (cid.cookie_id_path = [])) in
+        let strip uu___ =
+          match uu___ with | (cid, rslt) -> ((cid.cookie_id_key), rslt) in
+        FStar_List_Tot_Base.map strip
+          (FStar_List_Tot_Base.filter check b.browser_cookies)
+let (del_site_cookie :
+  BrowserIO.domain -> BrowserIO.path -> Prims.string -> browser -> browser) =
+  fun d ->
+    fun p ->
+      fun k ->
+        fun b ->
+          let cid =
+            { cookie_id_domain = d; cookie_id_path = p; cookie_id_key = k } in
+          {
+            browser_windows = (b.browser_windows);
+            browser_pages = (b.browser_pages);
+            browser_nodes = (b.browser_nodes);
+            browser_environments = (b.browser_environments);
+            browser_cookies = (remove_assoc cid b.browser_cookies);
+            browser_connections = (b.browser_connections)
+          }
+let rec (del_site_cookies :
+  BrowserIO.domain ->
+    BrowserIO.path -> Prims.string Prims.list -> browser -> browser)
+  =
+  fun d ->
+    fun p ->
+      fun ks ->
+        fun b ->
+          match ks with
+          | [] -> b
+          | k::ks1 ->
+              let b' = del_site_cookie d p k b in del_site_cookies d p ks1 b'
+let (set_site_cookie :
+  BrowserIO.domain ->
+    BrowserIO.path -> (Prims.string * Prims.string) -> browser -> browser)
+  =
+  fun d ->
+    fun p ->
+      fun uu___ ->
+        fun b ->
+          match uu___ with
+          | (k, v) ->
+              let cid =
+                { cookie_id_domain = d; cookie_id_path = p; cookie_id_key = k
+                } in
+              {
+                browser_windows = (b.browser_windows);
+                browser_pages = (b.browser_pages);
+                browser_nodes = (b.browser_nodes);
+                browser_environments = (b.browser_environments);
+                browser_cookies = (upd_assoc cid v b.browser_cookies);
+                browser_connections = (b.browser_connections)
+              }
+let rec (set_site_cookies :
+  BrowserIO.domain ->
+    BrowserIO.path ->
+      (Prims.string * Prims.string) Prims.list -> browser -> browser)
+  =
+  fun d ->
+    fun p ->
+      fun pairs ->
+        fun b ->
+          match pairs with
+          | [] -> b
+          | pair::pairs' ->
+              let b' = set_site_cookie d p pair b in
+              set_site_cookies d p pairs' b'
+let (upd_cookies :
+  BrowserIO.domain ->
+    BrowserIO.req_uri -> BrowserIO.resp -> browser -> browser)
+  =
+  fun d ->
+    fun uri ->
+      fun resp ->
+        fun b ->
+          let b' =
+            del_site_cookies d uri.BrowserIO.req_uri_path
+              resp.BrowserIO.resp_del_cookies b in
+          let b'' =
+            set_site_cookies d uri.BrowserIO.req_uri_path
+              resp.BrowserIO.resp_set_cookies b' in
+          b''
+let (http_send :
+  BrowserIO.domain ->
+    BrowserIO.req_uri ->
+      Prims.string -> dst -> browser -> (browser * BrowserIO.output_event))
+  =
+  fun d ->
+    fun uri ->
+      fun body ->
+        fun dst1 ->
+          fun b ->
+            let connections' = (d, uri, dst1) :: (b.browser_connections) in
+            let b' =
+              {
+                browser_windows = (b.browser_windows);
+                browser_pages = (b.browser_pages);
+                browser_nodes = (b.browser_nodes);
+                browser_environments = (b.browser_environments);
+                browser_cookies = (b.browser_cookies);
+                browser_connections = connections'
+              } in
+            let req =
+              {
+                BrowserIO.req_uri = uri;
+                BrowserIO.req_cookies =
+                  (get_site_cookies d uri.BrowserIO.req_uri_path b);
+                BrowserIO.req_body = body
+              } in
+            (b', (BrowserIO.Network_send_event (d, req)))
