project/Browser.fst
@@ -58,7 +58,7 @@ type cookie_id = {
 type win = {
     win_name: win_name;
     (** The window's name. *)
-    win_opener: win_ref;
+    win_opener: win_opener;
     (** The window's opener. If window is opened by user then no window_ref. Else reference to window from where window is opened*)
     win_page: page_ref;
     (** The window's page. *)
@@ -78,11 +78,11 @@ type context={
     * expressions. *)
 
 type inner=
-| Scoped_expr: context -> expr inner-> inner
-(** [Scoped_expr(cxt, e)] is a subexpression that executes in a different
+| Scoped_expr of context * expr inner
+      (** [Scoped_expr(cxt, e)] is a subexpression that executes in a different
           context than the enclosing expression. *)
-
-| Value : value -> inner 
+| R of value
+    (** A final result. *)
 
 
 (* A type for the results of evaluating script expressions. *)
@@ -148,14 +148,13 @@ let prim2 (prim: string) (r1: value) (r2: value)
     | ("&&", Bool_value(bl1), Bool_value(bl2)) -> Bool_value(bl1 && bl2)
     | ("+", String_value(s1), String_value(s2)) -> String_value(s1 ^ s2)
     | ("*", Int_value(n1), Int_value(n2)) -> Int_value( (let open FStar.Mul in n1 * n2))
-    // (let open FStar.Mul in n1 * n2)
     | ("+", Int_value(n1), Int_value(n2)) -> Int_value(n1 + n2)
     | ("-", Int_value(n1), Int_value(n2)) -> Int_value(n1 - n2)
     | ("addtourl", Url_value(u), String_value(s)) -> Url_value
         ( match u with 
             | Blank_url -> Blank_url
-            | Http_url domain ({req_uri_path = path; req_uri_params = params}) ->
-                 Http_url domain ({req_uri_path = path;
+            | Http_url (domain, {req_uri_path = path; req_uri_params = params}) ->
+                 Http_url (domain, {req_uri_path = path;
                                     req_uri_params = params ^ "?t=" ^ s})
          )
     | (_, Error(_), _) -> r1
@@ -171,6 +170,7 @@ let prim2 (prim: string) (r1: value) (r2: value)
   : expr inner =
     let f = to_inner_expr in
     begin match e with
+    // ---TO DO--
     | X(_) ->  Null  (* unreachable case *)            // assert (False)    --TODO--
     | Null -> Null
     | Bool(b) -> Bool(b)
@@ -228,20 +228,29 @@ let prim2 (prim: string) (r1: value) (r2: value)
 (** A typf eor document node. *)
 
 type node=
-| Para_node: option elt_id -> string -> node
-
-| Link_node: option elt_id -> url -> string -> node
-
-| Text_node: option elt_id -> string -> list value -> node
-
-| Button_node: option elt_id -> string -> list value -> node
-
-| Remote_script_node: option elt_id -> url -> bool -> node 
-
-| Div_node: elt_id -> list node_ref -> node 
-(** Represents a sequence of nodes in the document. list contains references to the children*)
-
-| Inline_script_node: option elt_id -> expr False -> bool -> node
+    | Para_node of option elt_id * string
+      (** Represents a text node. *)
+    | Link_node of option elt_id * url * string
+      (** Represents a link node. *)
+    | Textbox_node of option elt_id * string *  list value
+      (** [Textbox_Node(id, text, handlers)] represents a text input box along
+          with its current handlers. *)
+    | Button_node of option elt_id * string * list value
+      (** [Button_node(id, button_text, handlers)] represents a button along
+          with its current handlers.  If a handler is a function closure, it
+          will be run by applying the function to the button node with
+          which it's associated.  If a handler is any other result, it will be a
+          no-op. *)
+    | Inl_script_node of option elt_id * expr unit * bool
+      (** Represents a script node with an inline script, along with a flag
+          that indicates whether or not the script has been queued for
+          execution. *)
+    | Rem_script_node of option elt_id * url * bool
+      (** Represents a script node that references an external script, along
+          with a flag that indicates whether or not the script has been
+          requested. *)
+    | Div_node of option elt_id * list node_ref
+      (** Represents a sequence of nodes in the document. *)
 
 
 (** The type of the objects in a page's queue of scripts to execute. *)
@@ -260,7 +269,7 @@ type page={
 
     page_environment: act_ref;
 
-    page_script: list queued_expr;
+    page_script_queue: list queued_expr;
 }
 
 (** The type of an activation record in the scripting language. *)
@@ -270,14 +279,18 @@ type act = {
     act_vars: list (var * value);
 }
 
-(* typf eor open network connection *)
-type open_connection=
-
-| Doc_connection: domain -> req_uri -> win_ref -> open_connection
-
-| Script_connection: domain -> req_uri -> page_ref -> node_ref -> open_connection
-
-| Xhr_connection: domain -> req_uri -> page_ref -> value -> open_connection
+  type dst =
+    | Xhr_dst of page_ref * value
+      (** [Xhr_dst(pr, f)] represents a requested script that should be supplied
+          as an argument to the closure [f] and run on the page referenced by
+          [pr]. *)
+    | Doc_dst of win_ref
+      (** [Doc_dst(wr)] represents a requested document that should replace
+          the contents of the window referenced by [wr]. *)
+    | Script_dst of page_ref * node_ref
+      (** [Script_dst(pr, dr)] represents a requested script that should be used
+          to replace a marker in the [page_script_queue] of the page referenced
+          by [pr]. *)
 
 
 (** The type of a script expression queued for execution. *)
@@ -286,6 +299,8 @@ type open_connection=
     task_expr: expr inner;
   }
 
+(** asserting that activation parent has lower reference number than
+activation record **)
 let b_act_ref_pred (r:act_ref) (a:act) : bool = 
     match a.act_parent with | None -> true | Some ap -> r > ap
 
@@ -296,20 +311,41 @@ let rec b_env_pred (l:list (act_ref * act)) : bool =
 
 type b_env = l:(list (act_ref * act)){b_env_pred l}
 
-  (** A typf eor the basic state of a browser. *)
+(** asserting that if node is of type divi, its list of node_ref has 
+higher reference numbers **)
+let rec node_list_check(l:list node_ref)(n: node_ref): bool=
+  match l with 
+  |[] -> true
+  | r::tl -> r > n && (node_list_check tl n)
+
+let b_node_ref_pred (r:node_ref)(n:node) : bool=
+  match n with
+  | Div_node(n) -> node_list_check (snd(n)) r
+  | _ -> true
+
+let rec b_node_pred (l:list (node_ref * node)) : bool=
+  match l with 
+  | [] -> true
+  | (r,n):: t1-> b_node_ref_pred r n && (b_node_pred t1)
+
+
+type b_nodes= l: (list(node_ref * node)){b_node_pred l}
+
+  
+(** A typf eor the basic state of a browser. *)
 type browser = {
 
     browser_windows: list (win_ref * win) ;
     
     browser_pages: list (page_ref * page);
    
-    browser_nodes: list (node_ref * node);
+    browser_nodes: b_nodes;
   
     browser_environments: b_env ;
    
     browser_cookies: list (cookie_id * string) ;
    
-    browser_connections: list open_connection ;
+    browser_connections: list (domain * req_uri * dst) ;
    
 }
 
@@ -362,12 +398,10 @@ type browser = {
   : option page =
     assoc pr b.browser_pages
 
-(** redundant **)
-
 (** [page_assoc_valid pr b] returns the [page] associated with [pr] in the
       page store of [b]. *)
   let page_assoc_valid (pr: page_ref) (b: browser
- {(Some? (assoc pr b.browser_pages))}) : page =
+    {(Some? (assoc pr b.browser_pages))}) : page =
 
   Some?.v (assoc pr b.browser_pages)
 
@@ -422,25 +456,17 @@ let win_valid (wr: win_ref) (b: browser)
       store of [b], if one exists. *)
   let win_assoc (wr: win_ref) (b: browser)
   : option win =
-    List.assoc wr b.browser_windows  
+    assoc wr b.browser_windows  
 
-(** redundant **)
-
-  // (** [win_assoc_valid wr b] returns the [win] associated with [wr] in the window
-  //     store of [b]. *)
-  // let win_assoc_valid (wr: win_ref) (b: browser)
-  // : win =
-  //     begin try List.assoc wr b.browser_windows with
-  //     | None -> assert false
-  //     end
-
+(** [win_assoc_valid wr b] returns the [win] associated with [wr] in the window
+      store of [b]. *)
 let win_assoc_valid (wr:win_ref) (b:browser
 {(Some? (assoc wr b.browser_windows))}) : win =
 
   Some?.v (assoc wr b.browser_windows)
 
-  (** [win_update wr w b] associates [wr] with the new window [w] in [b]. *)
-  let win_update (wr: win_ref) (w: win) (b: browser)
+(** [win_update wr w b] associates [wr] with the new window [w] in [b]. *)
+let win_update (wr: win_ref) (w: win) (b: browser)
   : browser =
     let windows' = upd_assoc wr w b.browser_windows in
     { b with browser_windows = windows' }
@@ -481,9 +507,9 @@ end
   (** [win_from_user_window uw b] returns a reference to the open window in [b]
       that corresponds to the domain and number given by [uw]. *)
 
-      // need to implement 
-// let win_from_user_window ((u, n): user_window) (b:browser
-// {(Some? (assoc w.win_page b.browser_windows))})
+    // --TO DO--
+assume val win_from_user_window (u n: user_window) (b:browser) : option win_ref
+// let win_from_user_window ((u, n): user_window) (b:browser)
 //   : option win_ref =
 //     let has_url (_, w) =
 //       ((page_assoc_valid w.win_page b).page_location = u) in 
@@ -498,25 +524,24 @@ end
   (** [win_to_user_window wr b] returns the user window description
       corresponding to the valid window reference [wr]. *)
 
-   
-// nned to implement
-
-  // let win_to_user_window (wr: win_ref) (b: b)
-  // : user_window =
-  //   let w = win_assoc_valid wr b in
-  //   let u = (page_assoc_valid w.win_page b).page_location in
-  //   let has_url (_, w) =
-  //     (page_assoc_valid w.win_page b).page_location = u
-  //   in
-  //   let windows' = List.filter has_url b.browser_windows in
-  //   let rec find wr ws n =
-  //     begin match ws with
-  //     | (wr', _) :: _ when wr' = wr -> n
-  //     | _ :: ws' -> find wr ws' (succ n)
-  //     | _ -> assert false
-  //     end
-  //   in
-  //   User_window(u, find wr windows' 0)
+// --- TO DO--
+// assume val win_to_user_window (wr: win_ref) (b: browser) : user_window
+// let win_to_user_window (wr: win_ref) (b: browser)
+//   : user_window =
+//     let w = win_assoc_valid wr b in
+//     let u = (page_assoc_valid w.win_page b).page_location in
+//     let has_url (_, w) =
+//       (page_assoc_valid w.win_page b).page_location = u
+//     in
+//     let windows' = filter has_url b.browser_windows in
+//     let rec find_pos wr ws n =
+//       begin match ws with
+//       | (wr', _) :: ws' -> if wr' = wr then n 
+//       else find_pos wr ws' n+1
+//       | _ -> admit()  // assert false   --TO DO--
+//       end
+//     in
+//     (u, find_pos wr windows' 0)
 
 
 (** {4 Browser node store} *)
@@ -532,16 +557,34 @@ end
 (** [node_assoc_valid dr b] returns the [node] associated with [dr] in the
       node store of [b]. *)
 
-      // need to implement
-  let node_assoc_valid (dr: node_ref) (b: browser
-  {(Some? (assoc dr b.browser_nodes))}) : node =
+      // ---TO DO---
+let rec node_assoc_valid_lemma (dr: node_ref) (b:b_nodes):
+  Lemma (requires (Some? (assoc dr b)))
+  (ensures (b_node_ref_pred dr (Some?.v (assoc dr b))))=
+  match b with
+  |[] -> ()
+  | (k,_)::tl -> if k=dr then () else node_assoc_valid_lemma dr tl
 
-  Some?.v (assoc dr b.browser_nodes)
+let node_assoc_valid (dr: node_ref) (b: browser {node_valid dr b}) : (n:node{b_node_ref_pred dr n}) =
+    node_assoc_valid_lemma dr b.browser_nodes;
+  match (assoc dr b.browser_nodes) with 
+  | Some v -> v
+
+
+let rec node_update_lemma (dr: node_ref) (dn: node{b_node_ref_pred dr dn}) (b:b_nodes):
+ Lemma (requires (b_node_ref_pred dr dn))
+ (ensures (b_node_pred (upd_assoc dr dn b)))=
+      begin match b with
+    | [] -> ()
+    | (k', d') :: b' -> if k' = dr then () else node_update_lemma dr dn b'
+    end
+
 
   (** [node_update dr dn b] associates [dr] with the node [dn] in [b]. *)
-  let node_update (dr: node_ref) (dn: node) (b: browser)
+  let node_update (dr: node_ref) (dn: node{b_node_ref_pred dr dn}) (b: browser)
   : browser =
     let nodes' = upd_assoc dr dn b.browser_nodes in
+    node_update_lemma dr dn b.browser_nodes;
     { b with browser_nodes = nodes' }
 
 (** [node_new dn b] adds [dn] to the node store of [b] and returns its
@@ -551,7 +594,7 @@ end
   let n_ref = 
   (if length (b.browser_nodes) >=1 then (fst (last b.browser_nodes))
   else 0) in
-    let nr = fresh_win_ref (n_ref) in
+    let nr = fresh_node_ref (n_ref) in
     let b' = node_update nr dn b in
     (nr, b')
 
@@ -574,7 +617,7 @@ let node_parent (dr: node_ref) (b: browser)
      in
     let is_node_parent (_, dn) =
       begin match dn with
-      | Div_node _ children -> mem dr children
+      | Div_node (_, children) -> mem dr children
       | _ -> false
       end
     in
@@ -588,14 +631,15 @@ let node_parent (dr: node_ref) (b: browser)
   end
 
   (** Finds the page displaying a node if there is one. *)
-  // ---TO DO --
-  // let rec node_page (dr: node_ref) (b: browser)
-  // : option page_ref =
-  //   begin match node_parent dr b with
-  //   | No_parent -> None
-  //   | Page_parent (pr) -> Some pr
-  //   | Parent_node (dr1) -> node_page dr1 b
-  //   end
+// ---TO DO --
+// assume val node_page (dr: node_ref) (b: browser): option page_ref
+  let rec node_page (dr: node_ref) (b: browser)
+  : option page_ref =
+    begin match node_parent dr b with
+    | No_parent -> None
+    | Page_parent (pr) -> Some pr
+    | Parent_node (dr1) -> node_page dr1 b
+    end
 
 
 (** {4 Browser activation record store and variables} *)
@@ -630,7 +674,7 @@ let rec act_update_lemma (ar: act_ref) (act: act{b_act_ref_pred ar act}) (b:b_en
     | (k', d') :: b' -> if k' = ar then () else act_update_lemma ar act b'
     end
 
- (** [act_update ar l act b] associates [ar] with the new domain [l]
+(** [act_update ar l act b] associates [ar] with the new domain [l]
       and the new activation record [act] in [b]. *)
   let act_update (ar: act_ref) (act: act{b_act_ref_pred ar act}) (b: browser)
   : browser =
@@ -651,6 +695,7 @@ let rec act_update_lemma (ar: act_ref) (act: act{b_act_ref_pred ar act}) (b:b_en
 
 (** [get_var x ar b] gets the result associated with [x] in [b] in the scope
       defined by [ar], if [x] exists in that scope. *)
+
   let rec get_var (x: var) (ar: act_ref) (b: browser)
   : option value =
   if act_valid ar b then
@@ -665,4 +710,1428 @@ let rec act_update_lemma (ar: act_ref) (act: act{b_act_ref_pred ar act}) (b:b_en
     end
   else None
 
+(** [create_var x r ar b] creates (or overwrites) the binding of [x]
+      with the rslt [r] in the activation record referenced by [ar] in
+      [b]. *)
+      // --- TO DO --
+  let create_var (x: var) (r: value) (ar: act_ref) (b: browser)
+  : option browser =
+   if (act_valid ar b) then
+    let act = act_assoc_valid ar b in
+    let data' = upd_assoc x r act.act_vars in
+    let act' = { act with act_vars = data' } in
+    Some (act_update ar act' b)
+  else None /// --TO DO --
 
+  (** [set_var x r ar b] updates the nearest enclosing binding of [x] (with
+      the rslt [r]) under the scope defined by [ar] in [b].  If no current
+      binding is found, a new binding is created in the outermost scope. *)
+
+let rec set_var (x: var) (r: value) (ar: act_ref) (b: browser)
+  : option browser =
+   if (act_valid ar b) then
+    let act = act_assoc_valid ar b in
+    begin match assoc x act.act_vars with
+    | None -> begin match act.act_parent with
+      | None -> create_var x r ar b
+      | Some(ar1) -> set_var x r ar1 b
+    end
+    | _ -> let data' = upd_assoc x r act.act_vars in
+      let act' = { act with act_vars = data' } in
+     Some(act_update ar act' b )
+     end
+  else None
+
+// (** {4 Browser cookie store} *)
+
+  (**/**)
+  (** [prefix xs ys] returns [true] if [xs] is a prefix of [ys] and [false]
+      otherwise. *)
+  let rec prefix (#a:eqtype) (xs: list a) (ys: list a)
+  : bool =
+    begin match (xs, ys) with
+    | ([], _) -> true
+    | (x :: xs', y :: ys') -> x = y && prefix xs' ys'
+    | (_, _) -> false
+    end
+
+  (** [get_site_cookies d p b] builds the mapping of cookie keys and values
+      that is specific for the domain [d] and the path [p] in [b]. *)
+  let get_site_cookies (d: domain) (p: path) (b: browser)
+  : list (string * string)=
+    let check (cid, _) =
+      (cid.cookie_id_domain = d &&
+        prefix cid.cookie_id_path p) ||
+        (prefix cid.cookie_id_domain d &&
+          cid.cookie_id_path = [])
+    in
+    let strip (cid, rslt) = (cid.cookie_id_key, rslt) in
+    map strip (filter check b.browser_cookies)
+
+
+(** [del_site_cookie d p k b] removes the mapping for of cookie key [k] for
+      the domain [d] and path [p] in [b]. *)
+  let del_site_cookie (d: domain) (p: path) (k: string) (b: browser)
+  : browser =
+    let cid = {
+      cookie_id_domain = d;
+      cookie_id_path = p;
+      cookie_id_key = k;
+    } in
+    { b with browser_cookies = remove_assoc cid b.browser_cookies }
+
+  (** [del_site_cookies d p ks b] removes the mapping of all of the cookies with
+      keys in [ks] from the cookie store for the domain [d] and path [p] in
+      [b]. *)
+  let rec del_site_cookies (d: domain) (p: path) (ks: list string) (b: browser)
+  : browser =
+    begin match ks with
+    | [] -> b
+    | k :: ks1 ->
+        let b' = del_site_cookie d p k b in
+        del_site_cookies d p ks1 b'
+    end
+
+  (** [set_site_cookie d p (k, v) b] adds the mapping of the cookie key [k] to
+      the rslt [v] for the domain [d] and path [p] in [b]. *)
+  let set_site_cookie (d: domain) (p: path) ((k, v): string * string) (b: browser)
+  : browser =
+    let cid = {
+      cookie_id_domain = d;
+      cookie_id_path = p;
+      cookie_id_key = k;
+    } in
+    { b with browser_cookies = upd_assoc cid v b.browser_cookies }
+
+  (** [set_site_cookies d p pairs b] adds all of the key-rslt mappings in
+      [pairs] to the cookie store for the domain [d] and path [p] in [b]. *)
+  let rec set_site_cookies
+    (d: domain) (p: path) (pairs: list (string * string)) (b: browser)
+  : browser =
+    begin match pairs with
+    | [] -> b
+    | pair :: pairs' ->
+        let b' = set_site_cookie d p pair b in
+        set_site_cookies d p pairs' b'
+    end
+
+  (** [upd_cookies d uri resp b] executes all of the cookie updates requested
+      by [resp], which was received in response to a request to [d] for
+      resource [req_uri]. *)
+  let upd_cookies (d: domain) (uri: req_uri) (resp: resp) (b: browser)
+  : browser =
+    let b' = del_site_cookies d uri.req_uri_path resp.resp_del_cookies b in
+    let b'' = set_site_cookies d uri.req_uri_path resp.resp_set_cookies b' in
+    b''
+
+//   (** {4 Browser network connections} *)
+
+//   (** [net_connection_domain_nth d n b] returns the [n]th [req_uri] and [dst]
+//       associated with [d] (based on the order in which they were opened) among
+//       the open network connections of [b], if one exists. *)
+//   let net_connection_domain_nth (d: domain) (n: nat) (b: browser)
+//   : option (req_uri * dst) =
+//     let test (d', _, _) = (d' = d) in
+//     let connections' = filter test b.browser_connections in
+//     begin if length connections' <= n then
+//       None
+//     else
+//       let (_, uri, dst) = index connections' n in
+//       Some((uri, dst))
+//     end
+
+//   (** [net_connection_domain_remove_nth d n b] removes the [n]th [req_uri] and
+//       [dst] associated with [d] (based on the order in which they were opened)
+//       among the open network connections of [b], if one exists. *)
+//   // --TO DO ---
+// assume val net_connection_domain_remove_nth (d: domain) (n: nat) (b: browser): browser 
+//   // let net_connection_domain_remove_nth (d: domain) (n: nat) (b: browser)
+//   // : browser =
+//   //   let rec remove n cs =
+//   //     begin match cs with
+//   //     | [] -> []
+//   //     | (d',_,_) :: cs'-> if n = 0 && d' = d then cs' 
+//   //                           else if d' = d then (d',_,_):: remove (n-1) cs'
+//   //                           else (d',_,_) :: remove n cs'
+//   //     end
+//   //   in
+//   //   let connections' = remove n b.browser_connections in
+//   //   { b with browser_connections = connections' }
+
+  
+ (** [http_send d uri body dst b] updates the appropriate browser structures
+      and creates the necessary output events for sending a new HTTP request
+      whose response will be received by [dst]. *)
+  let http_send (d: domain) (uri: req_uri) (body: string) (dst: dst) (b: browser)
+  : browser * output_event =
+    let connections' = (d, uri, dst) :: b.browser_connections in
+    let b' = {
+      b with browser_connections = connections';} in
+    let req = {
+      req_uri = uri;
+      req_cookies = get_site_cookies d uri.req_uri_path b;
+      req_body = body;
+    } in
+    (b', Network_send_event(d, req))
+
+//  (** {3 Rendering documents for user output} *)
+
+//   // (**/**)
+//   //  --- TO DO ---
+
+//   assume val render_doc_as_list (dr: node_ref) (b: browser): list rendered_doc
+//   let rec render_doc_as_list (dr: node_ref) (b: browser)
+//   : list rendered_doc =
+//     assert (node_valid dr b);
+//     begin match node_assoc_valid dr b with
+//     | Para_node ( _, txt) -> [ Para_rendered(txt) ]
+//     | Link_node (_, u, txt) -> [ Link_rendered(u, txt) ]
+//     | Textbox_node (_, txt, _) -> [ Textbox_rendered(txt) ]
+//     | Button_node(_, txt, _) -> [ Button_rendered(txt) ]
+//     | Inl_script_node(_, _, _) -> []
+//     | Rem_script_node(_, _, _) -> []
+//     | Div_node(_, drs) ->
+//         let bd dr = render_doc_as_list dr b in
+//         [ Div_rendered(flatten (map bd drs)) ]
+//     end
+//   (**/**)
+
+
+//   // (** [render_page pr b] returns the rendered representation of the document in
+//   //     [pr].  A result of [None] indicates there are no visible contents.  The
+//   //     behavior of this function is undefined if [pr] is not a valid page
+//   //     reference. *)
+// assume val render_page (pr: page_ref) (b: browser)
+//   : option rendered_doc 
+//   // --- TO DO --
+//   // let render_page (pr: page_ref) (b: b)
+//   // : rendered_doc option =          
+//   //   assert (page_valid pr b);    
+//   //   begin match (page_assoc_valid pr b).page_document with
+//   //   | None -> None
+//   //   | Some(dr) ->
+//   //       begin match render_doc_as_list dr b with
+//   //       | [] -> None
+//   //       | rd :: _ -> Some(rd)
+//   //       end
+//   //   end
+
+
+//     (** [page_update_event pr b] returns a [UI_page_updated_event] for the page
+//       reference [pr]. *)
+// // --- TO DO ---
+// assume val page_update_event (pr: page_ref) (b: browser): output_event
+//   // let page_update_event (pr: page_ref) (b: browser)
+//   // : output_event =
+//   //   let wr =
+//   //     begin match page_win pr b with
+//   //     | None -> assert false
+//   //     | Some(wr) -> wr
+//   //     end
+//   //   in
+//   //   let uw = win_to_user_window wr b in
+//   //   let rd_opt = render_page pr b in
+//   //   UI_page_updated_event(uw, rd_opt)
+
+
+//   (** [build_win wn u doc b] builds a new window structure with the window name
+//       [wn].  A new page is created in [b] using [u] for the page's
+//       location.  If the contents can be displayed immediately, then a new
+//       activation record is also created for the window's environment. *)
+//   let build_win
+//     (wn: win_name) (u: url) (wo: win_opener) (doc: option node_ref) (b: browser)
+//   : win * browser =
+//     let a = {
+//       act_parent = None;
+//       act_vars = [];
+//     } in
+//     let (ar, b') = act_new a b in
+//     let p = {
+//       page_location = u;
+//       page_document = doc;
+//       page_environment = ar;
+//       page_script_queue = [];
+//     } in
+//     let (pr, b'') = page_new p b' in
+//     let w = {
+//       win_name = wn;
+//       win_opener = wo;
+//       win_page = pr;
+//     } in
+//     (w, b'')
+
+//   (** [fetch_url u wr b] performs whatever action is required by the URL [u]. *)
+//   //  --- TO DO --
+//   let fetch_url (u: url) (wr: win_ref) (b: browser)
+//   : browser * list output_event =
+//    assume (win_valid wr b);
+//     assert (win_valid wr b);
+//     begin match u with
+//     | Blank_url ->
+//         (b, [])
+//     | Http_url(d, uri) ->
+//         let dst = Doc_dst(wr) in
+//         let (b', oe) = http_send d uri "" dst b in
+//         (b', [ oe ])
+//     end
+
+//   (** [open_win wn u b] creates a new window in the browser with the window
+//       name [wn], directed to the URL [u].  It returns a reference to the newly
+//       created window. *)
+
+//   let open_win (wn: win_name) (u: url) (wo: win_opener) (b: browser)
+//   : win_ref * browser * list output_event =
+//     let (w', b') = build_win wn Blank_url wo None b in
+//     let (wr, b'') = win_new w' b' in
+//     let (b''', oes) = fetch_url u wr b'' in
+//     (wr, b''', UI_win_opened_event :: oes)
+
+
+// (** [close_doc_request_connections wr b] removes any network connection
+//       that is waiting for a document to load into the window referenced by
+//       [wr]. *)
+//   let close_doc_request_connections (wr: win_ref) (b: browser)
+//   : browser =
+// // -- to do --
+//     assume (win_valid wr b);
+//     assert (win_valid wr b);
+//     let not_for_wr (_, _, dst) =
+//       begin match dst with
+//       | Doc_dst(wr') -> wr' <> wr
+//       | _ -> true
+//       end
+//     in
+//     let connections' = filter not_for_wr b.browser_connections in
+//     { b with browser_connections = connections' }
+
+//  (** [direct_win wr u b] directs the window referenced by [wr] to the URL
+//       [u]. *)
+//   let direct_win (wr: win_ref) (u: url) (b: browser)
+//   : browser * list output_event =
+// // -- to do --
+//     assume (win_valid wr b);
+//     assert (win_valid wr b);
+//     let b' = close_doc_request_connections wr b in
+//     begin match u with
+//     | Blank_url ->
+//         let uw = win_to_user_window wr b' in
+//         let w = win_assoc_valid wr b' in
+//         let b'1 = page_remove w.win_page b' in
+//         let (w', b'2) = build_win w.win_name Blank_url w.win_opener None b'1 in
+//         let b'3 = win_update wr w' b'2 in
+//         let oe = UI_page_loaded_event(uw, Blank_url, None) in
+//         (b'3, [ oe ])
+//     | _ ->
+//         fetch_url u wr b
+//     end
+
+
+//   (** {3 Node tree operations} *)
+
+//   (** [build_node_tree doc] allocates all of the node references needed to
+//       represent [doc] and returns the association list of these nodes with their
+//       appropriate node data.  It also returns the reference to the root of the
+//       node tree that was created. *)
+
+//   // let rec build_node_tree (doc: doc)
+//   // : node_ref * list (node_ref * node) =
+
+//   // // ---TO DO Recursion error--
+
+//   //   let dr = fresh_node_ref 0 in  // what to do give input? in fresh_node_ref()
+//   //   match doc with
+//   //   | Para(id, text) ->
+//   //       (dr, [ (dr, Para_node(id, text)) ])
+//   //   | Link(id, u, text) ->
+//   //       (dr, [ (dr, Link_node(id, u, text)) ])
+//   //   | Textbox(id, text) ->
+//   //       (dr, [ (dr, Textbox_node(id, text, [])) ])
+//   //   | Button(id, text) ->
+//   //       (dr, [ (dr, Button_node(id, text, [])) ])
+//   //   | Inl_script(id, e) ->
+//   //       (dr, [ (dr, Inl_script_node(id, e, false)) ])
+//   //   | Rem_script(id, u) ->
+//   //       (dr, [ (dr, Rem_script_node(id, u, false)) ])
+//   //   | Divi(id, subdocs) ->
+//   //       let (drs, nhs) = split (map build_node_tree subdocs) in
+//   //       (dr, (dr, Div_node(id, drs)) :: flatten nhs)
+
+
+//   (** [split_queued_exprs qes] returns the prefix of [qes] that are known
+//       scripts, as an [inner expr list], along with the remainder of [qes]. *)
+  
+//   // --- TO DO -- TYPE ERROR
+  
+//   // let split_queued_exprs (qes: list queued_expr)
+//   // : (list expr inner) * (list queued_expr)  =
+//   //   let rec take_ready qes =
+//   //     begin match qes with
+//   //     | Known_expr(e) :: ps1 -> e :: take_ready ps1
+//   //     | _ -> []
+//   //     end
+//   //   in
+//   //   let rec drop_ready qes =
+//   //     begin match qes with
+//   //     | Known_expr(e) :: ps1 -> drop_ready ps1
+//   //     | _ -> qes
+//   //     end
+//   //   in
+//   //   (take_ready qes, drop_ready qes)
+
+
+//   // (**/**)
+//   // let rec process_node_scripts_aux (pr: page_ref) (dr: node_ref) (b: browser)
+//   // : browser * list queued_expr * list output_event =
+
+//   // // -- TO DO --
+//   //   assume (page_valid pr b);
+//   //   assume (node_valid dr b);
+//   //   assert (page_valid pr b);
+//   //   assert (node_valid dr b);
+//   //   begin match node_assoc_valid dr b with
+//   //   | Para_node(_, _)
+//   //   | Link_node(_, _, _)
+//   //   | Textbox_node(_, _, _)
+//   //   | Button_node(_, _, _)
+//   //   | Inl_script_node(_, _, true)
+//   //   | Rem_script_node(_, _, true)
+//   //   | Rem_script_node(_, Blank_url, _) ->
+//   //       (b, [], [])
+//   //   | Inl_script_node(id, e, false) ->
+//   //       let b' = node_update dr (Inl_script_node(id, e, true)) b in
+//   //       (b', [ Known_expr(to_inner_expr e) ], [])
+//   //   | Rem_script_node(id, Http_url(d, uri), false) ->
+//   //       let b' = node_update dr (Rem_script_node(id, Http_url(d, uri), true)) b in
+//   //       let (b'', oe) = http_send d uri "" (Script_dst(pr, dr)) b' in
+//   //       (b'', [ Unknown_expr(dr) ], [ oe ])
+//   //   | Div_node(_, drs) ->
+//   //       process_node_scripts_list pr drs b
+//   //   end
+
+//   // and process_node_scripts_list (pr: page_ref) (drs: list node_ref) (b: browser)
+//   // : browser * list queued_expr * list output_event =
+//   //   begin match drs with
+//   //   | [] -> (b, [], [])
+//   //   | dr' :: drs' ->
+//   //       let (b', pes1, oes1) = process_node_scripts_aux pr dr' b in
+//   //       let (b'', pes2, oes2) = process_node_scripts_list pr drs' b' in
+//   //       (b'', pes1 @ pes2, oes1 @ oes2)
+//   //   end
+//   // (**/**)
+
+// //   (** [process_node_scripts pr dr b] prepares for execution all of the scripts
+// //       that are found among the descendents of [dr] and have not yet been
+// //       executed.  (Preparing them for execution means putting them in the proper
+// //       queue.)  It also generates network requests for all of the remote
+// //       scripts that have not been requested. *)
+// //   let rec process_node_scripts (pr: page_ref) (dr: node_ref) (b: browser)
+// //   : browser * list output_event * list task =
+// //     assert (page_valid pr b);
+// //     assert (node_valid dr b);
+// //     let (b', qes, oes) = process_node_scripts_aux pr dr b in
+// //     begin match page_win pr b with
+// //     | None ->
+// //         (b', oes, [])
+// //     | Some(wr) ->
+// //         let p = page_assoc_valid pr b' in
+// //         let (exprs, qes') = split_queued_exprs (p.page_script_queue @ qes) in
+// //         let p' = { p with page_script_queue = qes' } in
+// //         let b'' = page_update pr p' b' in
+// //         let task e = {
+// //           task_win = wr;
+// //           task_expr = e;
+// //         } in
+// //         (b'', oes, List.map task exprs)
+// //     end
+
+//   (**/**)
+//   let rec textbox_handlers_in_tree dr b =
+//     begin match node_assoc_valid dr b with
+//     | Para_node(_, _)
+//     | Link_node(_, _, _)
+//     | Button_node(_, _, _)
+//     | Inl_script_node(_, _, _)
+//     | Rem_script_node(_, _, _) ->
+//         []
+//     | Textbox_node(_, _, handlers) ->
+//         [ (dr, handlers) ]
+//     | Div_node(_, drs) ->
+//         flatten (map (fun dr -> textbox_handlers_in_tree dr b) drs)
+//     end
+
+
+//   let rec button_handlers_in_tree dr b =
+//     begin match node_assoc_valid dr b with
+//     | Para_node(_, _)
+//     | Link_node(_, _, _)
+//     | Textbox_node(_, _, _)
+//     | Inl_script_node(_, _, _)
+//     | Rem_script_node(_, _, _) ->
+//         []
+//     | Button_node(_, _, handlers) ->
+//         [ (dr, handlers) ]
+//     | Div_node(_, drs) ->
+//         flatten (map (fun dr -> button_handlers_in_tree dr b) drs)
+//     end
+
+//   (** [textbox_handlers_in_pos wr pos b] returns the textbox handlers associated
+//       with the textbox in position [pos] in the window referenced by [wr] in
+//       [b], along with the corresponding [node_ref]. *)
+// //   let textbox_handlers_in_pos (wr: win_ref) (posi: int) (b: browser)
+// //   : option (node_ref * list value) =
+// //     assert (win_valid wr b);
+// //     begin match
+// //       (page_assoc_valid (win_assoc_valid wr b).win_page b).page_document
+// //     with
+// //     | None -> None
+// //     | Some(root) ->
+// //         begin try
+// //           Some(index (textbox_handlers_in_tree root b) posi)
+// //         with
+// //         | Failure("nth") -> None
+// //         end
+// //     end
+
+//   (** [button_handlers_in_pos wr pos b] returns the button handlers associated
+//       with the button in position [pos] in the window referenced by [wr] in
+//       [b], along with the corresponding [node_ref]. *)
+// //   let button_handlers_in_pos (wr: win_ref) (posi: int) (b: browser)
+// //   : option (node_ref * list value) =
+// //     assert (win_valid wr b);
+// //     begin match
+// //       (page_assoc_valid (win_assoc_valid wr b).win_page b).page_document
+// //     with
+// //     | None -> None
+// //     | Some(root) ->
+// //         begin try
+// //           Some(index (button_handlers_in_tree root b) posi)
+// //         with
+// //         | Failure("nth") -> None
+// //         end
+// //     end
+
+//   (** {3 Inserting and removing document nodes} *)
+
+//   (** Removes a node from its location in its node tree or page. *)
+//   let node_remove (dr: node_ref) (b: browser)
+//   : b * output_event list =
+//     begin match node_parent dr b with
+//     | No_parent ->
+//         (b, [])
+//     | Page_parent(pr') ->
+//         let p = page_assoc_valid pr' b in
+//         let p' = { p with page_document = None } in
+//         let b' = page_update pr' p' b in
+//         (b', [ page_update_event pr' b' ])
+//     | Parent_node(p) ->
+//         begin match node_assoc_valid p b with
+//         | Div_node(id, children) ->
+//             let children' = List.filter (fun dr' -> dr' <> dr) children in
+//             let b' = node_update p (Div_node(id, children')) b in
+//             begin match node_page dr b with
+//             | None -> (b', [])
+//             | Some(pr') -> (b', [ page_update_event pr' b' ])
+//             end
+//         | _ -> assert false
+//         end
+//     end
+
+//   (**/**)
+//   (** Computes the set of all descendents of a node. *)
+//   let rec node_descendents (strict: bool) (dr: node_ref) (b: browser)
+//   : node_ref list =
+//     assert (node_valid dr b);
+//     begin match node_assoc_valid dr b with
+//     | Div_node(_, drs) ->
+//         let dd dr = node_descendents false dr b in
+//         begin if strict then
+//           List.flatten (List.map dd drs)
+//         else
+//           dr :: List.flatten (List.map dd drs)
+//         end
+//     | _ ->
+//         if strict then [] else [ dr ]
+//     end
+
+//   (** [insert_in_list x xs k] inserts [x] as the [k]th element of [xs]. *)
+//   let rec insert_in_list (x: 'a) (xs: 'a list) (k: int)
+//   : 'a list =
+//     begin match (xs, k) with
+//     | (xs, 0) -> x :: xs
+//     | (x' :: xs', k) when k > 0 -> x' :: insert_in_list x xs' (k-1)
+//     | (_, _) -> failwith "insert_in_list"
+//     end
+//   (**/**)
+
+//   (** [insert_node parent child pos b] inserts [child] into the children
+//       of [parent] at position [pos]. *)
+//   let node_insert (parent: node_ref) (child: node_ref) (pos: int) (b: browser)
+//   : b * output_event list * task list =
+//     assert (node_valid parent b);
+//     assert (node_valid child b);
+//     if List.mem parent (node_descendents true parent b) then
+//       failwith "node_insert";
+//     let (b', oes1) = node_remove child b in
+//     begin match node_assoc_valid parent b' with
+//     | Div_node(id, children) ->
+//         let children' = insert_in_list child children pos in
+//         let dn' = Div_node(id, children') in
+//         let b'' = node_update parent dn' b' in
+//         begin match node_page parent b'' with
+//         | None -> (b'', oes1, [])
+//         | Some(pr) ->
+//             let (b''', oes2, ts) = process_node_scripts pr child b'' in
+//             (b''', oes1 @ [ page_update_event pr b''' ] @ oes2, ts)
+//         end
+//     | _ -> failwith "node_insert"
+//     end 
+
+//   (** {3 Executing scripts} *)
+
+//   (**/**)
+//   (** Converts a [value] to a [elt_id], if possible. *)
+//   let rslt_to_elt_it_opt (r: value)
+//   : option elt_id =
+//     begin match r with
+//     | String_value(id) -> Some({ elt_id_value = id })
+//     | _ -> None
+//     end
+//   (**/**)
+
+//   (** Carries out a single step of executing a script expression. *)
+//   let rec step_expr (ctx: context) (b: browser) (e: expr inner)
+//   : browser * expr inner * list output_event * list task =
+//     let step = step_expr ctx in
+//     begin match e with
+
+//     (* error propagation rules: an expression with an error in a subexression
+//      * must step to an error *)
+
+//     | Eval(X(R(Error(s))))
+//     | Apply(X(R(Error(s))), _)
+//     | Prim1(_, X(R(Error(s))))
+//     | Prim2(_, X(R(Error(s))), _)
+//     | Alert(X(R(Error(s))))
+//     | If(X(R(Error(s))), _, _)
+//     | Set_var(_, X(R(Error(s))))
+//     | Seq(X(R(Error(s))), _)
+//     | Get_cookie(X(R(Error(s))), _)
+//     | Set_cookie(X(R(Error(s))), _, _)
+//     | Xhr(X(R(Error(s))), _, _)
+//     | Named_win(X(R(Error(s))))
+//     | Open_win(X(R(Error(s))))
+//     | Open_named_win(X(R(Error(s))), _)
+//     | Close_win(X(R(Error(s))))
+//     | Navigate_win(X(R(Error(s))), _)
+//     | Is_win_closed(X(R(Error(s))))
+//     | Get_win_opener(X(R(Error(s))))
+//     | Get_win_location(X(R(Error(s))))
+//     | Get_win_name(X(R(Error(s))))
+//     | Set_win_name(X(R(Error(s))), _)
+//     | Get_win_root_node(X(R(Error(s))))
+//     | Set_win_root_node(X(R(Error(s))), _)
+//     | Get_win_var(X(R(Error(s))), _)
+//     | Set_win_var(X(R(Error(s))), _, _)
+//     | New_node(X(R(Error(s))))
+//     | Get_node_type(X(R(Error(s))))
+//     | Get_node_contents(X(R(Error(s))))
+//     | Set_node_contents(X(R(Error(s))), _)
+//     | Get_node_attr(X(R(Error(s))), _)
+//     | Set_node_attr(X(R(Error(s))), _, _)
+//     | Remove_handlers(X(R(Error(s))))
+//     | Add_handler(X(R(Error(s))), _)
+//     | Get_parent(X(R(Error(s))))
+//     | Get_child(X(R(Error(s))), _)
+//     | Insert_node(X(R(Error(s))), _, _)
+//     | Remove_node(X(R(Error(s)))) ->
+
+//       (b, X(R(Error(s))), [], [])
+
+//     | Apply(X(R(_)), X(R(Error(s))))
+//     | Prim2(_, X(R(_)), X(R(Error(s))))
+//     | Get_cookie(X(R(_)), X(R(Error(s))))
+//     | Set_cookie(X(R(_)), X(R(Error(s))), _)
+//     | Open_named_win(X(R(_)), X(R(Error(s))))
+//     | Navigate_win(X(R(_)), X(R(Error(s))))
+//     | Set_node_contents(X(R(_)), X(R(Error(s))))
+//     | Get_node_attr(X(R(_)), X(R(Error(s))))
+//     | Set_node_attr(X(R(_)), X(R(Error(s))), _)
+//     | Set_win_name(X(R(_)), X(R(Error(s))))
+//     | Set_win_root_node(X(R(_)), X(R(Error(s))))
+//     | Set_win_var(X(R(_)), _, X(R(Error(s))))
+//     | Add_handler(X(R(_)), X(R(Error(s))))
+//     | Get_child(X(R(_)), X(R(Error(s))))
+//     | Insert_node(X(R(_)), X(R(Error(s))), _)
+//     | Xhr(X(R(_)), X(R(Error(s))), _) ->
+
+//         (b, X(R(Error(s))), [], [])
+
+//     | Set_cookie(X(R(_)), X(R(_)), X(R(Error(s))))
+//     | Xhr(X(R(_)), X(R(_)), X(R(Error(s))))
+//     | Set_node_attr(X(R(_)), X(R(_)), X(R(Error(s))))
+//     | Insert_node(X(R(_)), X(R(_)), X(R(Error(s)))) ->
+
+//         (b, X(R(Error(s))), [], [])
+
+//     (* computational rules *)
+
+//     | X(R(_)) ->
+//         (* this should only be reached in the case of a runtime type error *)
+//         let err = "run-time type error" in
+//         (b, X(R(Error(err))), [], [])
+
+//     | X(Scoped_expr(_, X(R(r1)))) ->
+//         (b, X(R(r1)), [], [])
+//     | X(Scoped_expr(ctx', e1)) ->
+//         let (b', e1', oes, ts) = step_expr ctx' b e1 in
+//         (b', X(Scoped_expr(ctx', e1')), oes, ts)
+
+//     | Null ->
+//         (b, X(R(Null_value)), [], [])
+//     | Bool(bl) ->
+//         (b, X(R(Bool_value(bl))), [], [])
+//     | Int(n) ->
+//         (b, X(R(Int_value(n))), [], [])
+//     | String(s) ->
+//         (b, X(R(String_value(s))), [], [])
+//     | Url(u) ->
+//         (b, X(R(Url_value(u))), [], [])
+//     | Types(t) ->
+//         (b, X(R(Type_value(t))), [], [])
+
+//     | Code(e) ->
+//         (b, X(R(Code_value(e))), [], [])
+//     | Eval(X(R(Code_value(e1)))) ->
+//         (b, to_inner_expr e1, [], [])
+
+//     | Var(x) ->
+//         begin match get_var x ctx.context_act b with
+//         | None ->
+//             let err = Printf.sprintf "variable %S not found" x.var_name in
+//             (b, X(R(Error(err))), [], [])
+//         | Some(r) ->
+//             (b, X(R(r)), [], [])
+//         end
+
+//     | Function(x, locals, e1) ->
+//         (b, X(R(Closure(ctx, x, locals, e1))), [], [])
+//     | Apply(X(R(Closure(ctx1, x, locals, e1))), X(R(r2))) ->
+//         let bot_null x = (x, Null_value) in
+//         let act = {
+//           act_parent = Some(ctx1.context_act);
+//           act_vars = (x, r2) :: List.map bot_null locals;
+//         } in
+//         let (ar', b') = act_new act b in
+//         let ctx2 = { ctx1 with context_act = ar' } in
+//         (b', X(Scoped_expr(ctx2, e1)), [], [])
+
+//     | Prim1(prim, X(R(r))) ->
+//         (b, X(R(prim1 prim r)), [], [])
+//     | Prim2(prim, X(R(r1)), X(R(r2))) ->
+//         (b, X(R(prim2 prim r1 r2)), [], [])
+//     | Alert(X(R(Null_value))) ->
+//         (b, X(R(Null_value)), [ UI_alert("null") ], [])
+//     | Alert(X(R(Bool_value(bl)))) ->
+//         (b, X(R(Null_value)), [ UI_alert(Printf.sprintf "%B" bl) ], [])
+//     | Alert(X(R(Int_value(n)))) ->
+//         (b, X(R(Null_value)), [ UI_alert(Printf.sprintf "%N" n) ], [])
+//     | Alert(X(R(String_value(s)))) ->
+//         (b, X(R(Null_value)), [ UI_alert(s) ], [])
+//     | Alert(X(R(Url_value(_)))) ->
+//         (b, X(R(Null_value)), [ UI_alert("<URL>") ], [])
+//     | Alert(X(R(Code_value(_)))) ->
+//         (b, X(R(Null_value)), [ UI_alert("<code>") ], [])
+//     | Alert(X(R(Win_value(_)))) ->
+//         (b, X(R(Null_value)), [ UI_alert("<window>") ], [])
+//     | Alert(X(R(Node_value(_)))) ->
+//         (b, X(R(Null_value)), [ UI_alert("<node>") ], [])
+//     | Alert(X(R(Closure(_, _, _, _)))) ->
+//         (b, X(R(Null_value)), [ UI_alert("<function>") ], [])
+
+//     | Set_var(x, X(R(r1))) ->
+//         (set_var x r1 ctx.context_act b, X(R(r1)), [], [])
+//     | If(X(R(Bool_value(true))), e2, e3) ->
+//         (b, e2, [], [])
+//     | If(X(R(Bool_value(false))), e2, e3) ->
+//         (b, e3, [], [])
+//     | While(e1, e2) ->
+//         (b, If(e1, Seq(e2, While(e1, e2)), Null), [], [])
+//     | Seq(X(R(_)), e2) ->
+//         (b, e2, [], [])
+
+//     // | Get_cookie(X(R(Url_value(Http_url(d, uri)))), X(R(String_value(ck)))) ->
+//     //     let cs = get_site_cookies d uri.req_uri_path b in
+//     //     begin try
+//     //       (b, X(R(String_value(List.assoc ck cs))), [], [])
+//     //     with
+//     //     | Not_found -> (b, X(R(Null_value)), [], [])
+//     //     end
+//     | Set_cookie(
+//           X(R(Url_value(Http_url(d, uri)))),
+//           X(R(String_value(ck))),
+//           X(R(Null_value))) ->
+//         let b' = del_site_cookie d uri.req_uri_path ck b in
+//         (b', X(R(Null_value)), [], [])
+//     | Set_cookie(
+//           X(R(Url_value(Http_url(d, uri)))),
+//           X(R(String_value(ck))),
+//           X(R(String_value(cv)))) ->
+//         let b' = set_site_cookie d uri.req_uri_path (ck, cv) b in
+//         (b', X(R(Null_value)), [], [])
+
+//     | Xhr(X(R(Url_value(Blank_url))), X(R(_)), X(R(_))) ->
+//         (b, X(R(Null_value)), [], [])
+//         (* XXX: perhaps this should be an error, rather than a no-op *)
+
+//     | Xhr(X(R(Url_value(Http_url(d, uri)))),
+//           X(R(String_value(msg))), X(R(Closure(_, _, _, _)))) ->
+//         begin if not (win_valid ctx.context_win b) then
+//           let err = "window was closed---cannot make AJAX request" in
+//           (b, X(R(Error(err))), [], [])
+//         else
+//           let w = win_assoc_valid ctx.context_win b in
+//           let dst = Xhr_dst(w.win_page, Closure(_, _, _, _)) in
+//           let (b', oe) = http_send d uri msg dst b in
+//           (b', X(R(Null_value)), [ oe ], [])
+//         end
+
+//     | Self_win ->
+//         (* In some browsers, it may be an error to evaluate "self" if the
+//            original window is no longer open.  Here we let "self" evaluate to an
+//            invalid window reference, but an error will occur if this reference
+//            is ever used, except to test whether it has been closed. *)
+//         (b, X(R(Win_value(ctx.context_win))), [], [])
+
+//     | Named_win(X(R(String_value(wn)))) ->
+//         begin match win_from_win_name wn b with
+//         | None -> (b, X(R(Null_value)), [], [])
+//         | Some(wr) -> (b, X(R(Win_value(wr))), [], [])
+//         end
+
+//     | Open_win(X(R(Url_value(u)))) ->
+//         let wo = Win_opener(ctx.context_win) in
+//         let (wr, b', oes) = open_win No_name u wo b in
+//         (b', X(R(Win_value(wr))), oes, [])
+//     | Open_named_win(X(R(Url_value(u))), X(R(String_value(str)))) ->
+//         begin match win_from_win_name str b with
+//         | None ->
+//             let wo = Win_opener(ctx.context_win) in
+//             let (wr, b', oes) = open_win (Str_name(str)) u wo b in
+//             (b', X(R(Win_value(wr))), oes, [])
+//         | Some(wr) ->
+//             let (b', oes) = direct_win wr u b in
+//             (b', X(R(Win_value(wr))), oes, [])
+//         end
+//     | Close_win(X(R(Win_value(wr)))) ->
+//         let oes =
+//           if win_valid wr b then [ UI_win_closed_event(win_to_user_window wr b) ]
+//           else []
+//         in
+//         (win_remove wr b, X(R(Null_value)), oes, [])
+//     | Navigate_win(
+//           X(R(Win_value(wr))),
+//           X(R(Url_value(url)))) ->
+//         begin if win_valid wr b then
+//           let (b', oes) = direct_win wr (url) b in
+//           (b', X(R(Null_value)), oes, [])
+//         else
+//           let err = "window was closed---cannot set location" in
+//           (b, X(R(Error(err))), [], [])
+//         end
+
+//     | Is_win_closed(X(R(Win_value(wr)))) ->
+//         (b, X(R(Bool_value(not (win_valid wr b)))), [], [])
+//     | Get_win_opener(X(R(Win_value(wr)))) ->
+//         begin match win_assoc wr b with
+//         | None ->
+//             let err = "window was closed---cannot get opener" in
+//             (b, X(R(Error(err))), [], [])
+//         | Some(w) ->
+//             begin match w.win_opener with
+//             | No_opener -> (b, X(R(Null_value)), [], [])
+//             | Win_opener(wr') -> (b, X(R(Win_value(wr))), [], [])
+//             end
+//         end
+//     | Get_win_location(X(R(Win_value(wr)))) ->
+//         begin match win_assoc wr b with
+//         | None ->
+//             let err = "window was closed---cannot get location" in
+//             (b, X(R(Error(err))), [], [])
+//         | Some(w) ->
+//             let u =
+//               (page_assoc_valid w.win_page b).page_location
+//             in
+//             (b, X(R(Url_value(u))), [], [])
+//         end
+
+//     | Get_win_name(X(R(Win_value(wr)))) ->
+//         begin match win_assoc wr b with
+//         | None ->
+//             let err = "window was closed---cannot get name" in
+//             (b, X(R(Error(err))), [], [])
+//         | Some(w) ->
+//             begin match w.win_name with
+//             | No_name ->
+//                 (b, X(R(Null_value)), [], [])
+//             | Str_name(str) ->
+//                 (b, X(R(String_value(str))), [], [])
+//             end
+//         end
+
+//     | Set_win_name(X(R(Win_value(wr))), X(R(Null_value))) ->
+//         begin match win_assoc wr b with
+//         | None ->
+//             let err = "window was closed---cannot unset name" in
+//             (b, X(R(Error(err))), [], [])
+//         | Some(w) ->
+//             let w' = { w with win_name = No_name } in
+//             let b' = win_update wr w' b in
+//             (b', X(R(Null_value)), [], [])
+//         end
+//     | Set_win_name(X(R(Win_value(wr))), X(R(String_value(str)))) ->
+//         begin match win_assoc wr b with
+//         | None ->
+//             let err = "window was closed---cannot set name" in
+//             (b, X(R(Error(err))), [], [])
+//         | Some(w) ->
+//             let w' = { w with win_name = Str_name(str) } in
+//             let b' = win_update wr w' b in
+//             (b', X(R(Null_value)), [], [])
+//         end
+
+//     | Get_win_root_node(X(R(Win_value(wr)))) ->
+//         begin match win_assoc wr b with
+//         | None ->
+//             let err = "window was closed---cannot get root node" in
+//             (b, X(R(Error(err))), [], [])
+//         | Some(w) ->
+//             begin match (page_assoc_valid w.win_page b).page_document with
+//             | None ->
+//                 (b, X(R(Null_value)), [], [])
+//             | Some(dr) ->
+//                 (b, X(R(Node_value(dr))), [], [])
+//             end
+//         end
+//     | Set_win_root_node(
+//           X(R(Win_value(wr))),
+//           X(R(Node_value(dr)))) ->
+//         begin match win_assoc wr b with
+//         | None ->
+//             let err = "window was closed---cannot set root node" in
+//             (b, X(R(Error(err))), [], [])
+//         | Some(w) ->
+//             let (b', oes1) = node_remove dr b in
+//             let p = page_assoc_valid w.win_page b in
+//             let p' = { p with page_document = Some(dr) } in
+//             let b'' = page_update w.win_page p' b' in
+//             let (b''', oes2, ts) = process_node_scripts w.win_page dr b'' in
+//             let oes = oes1 @ [ page_update_event w.win_page b''' ] @ oes2 in
+//             (b''', X(R(Null_value)), oes, ts)
+//         end
+
+//     | Get_win_var(X(R(Win_value(wr))), x) ->
+//         begin match win_assoc wr b with
+//         | None ->
+//             let err =
+//               Printf.sprintf "window was closed---cannot get variable %S"
+//                 x.var_name
+//             in
+//             (b, X(R(Error(err))), [], [])
+//         | Some(w) ->
+//             let ar = (page_assoc_valid w.win_page b).page_environment in
+//             begin match get_var x ar b with
+//             | None ->
+//                 let err =
+//                   Printf.sprintf "window variable %S not found" x.var_name
+//                 in
+//                 (b, X(R(Error(err))), [], [])
+//             | Some(r) ->
+//                 (b, X(R(r)), [], [])
+//             end
+//         end
+//     | Set_win_var(X(R(Win_value(wr))), x, X(R(r2))) ->
+//         begin match win_assoc wr b with
+//         | None ->
+//             let err =
+//               Printf.sprintf "window was closed---cannot set variable %s"
+//                 x.var_name
+//             in
+//             (b, X(R(Error(err))), [], [])
+//         | Some(w) ->
+//             let ar = (page_assoc_valid w.win_page b).page_environment in
+//             let b' = set_var x r2 ar b in
+//             (b', X(R(Null_value)), [], [])
+//         end
+
+//     | New_node(X(R(String_value("para")))) ->
+//         let (dr, b') = node_new (Para_node(None, "")) b in
+//         (b', X(R(Node_value(dr))), [], [])
+
+//     | New_node(X(R(String_value("link")))) ->
+//         let (dr, b') = node_new (Link_node(None, Blank_url, "")) b in
+//         (b', X(R(Node_value(dr))), [], [])
+
+//     | New_node(X(R(String_value("textbox")))) ->
+//         let (dr, b') = node_new (Textbox_node(None, "", [])) b in
+//         (b', X(R(Node_value(dr))), [], [])
+
+//     | New_node(X(R(String_value("button")))) ->
+//         let (dr, b') = node_new (Button_node(None, "", [])) b in
+//         (b', X(R(Node_value(dr))), [], [])
+
+//     | New_node(X(R(String_value("inl_script")))) ->
+//         let (dr, b') = node_new (Inl_script_node(None, Null, false)) b in
+//         (b', X(R(Node_value(dr))), [], [])
+
+//     | New_node(X(R(String_value("rem_script")))) ->
+//         let (dr, b') = node_new (Rem_script_node(None, Blank_url, false)) b in
+//         (b', X(R(Node_value(dr))), [], [])
+
+//     | New_node(X(R(String_value("div")))) ->
+//         let (dr, b') = node_new (Div_node(None, [])) b in
+//         (b', X(R(Node_value(dr))), [], [])
+
+//     | New_node(X(R(String_value(_)))) ->
+//         let err = "expected valid node type string" in
+//         (b, X(R(Error(err))), [], [])
+
+//     | Get_node_type(X(R(Node_value(dr)))) ->
+//         begin match node_assoc_valid dr b with
+//         | Para_node(_, _) ->
+//             (b, X(R(String_value("para"))), [], [])
+//         | Link_node(_, _, _) ->
+//             (b, X(R(String_value("link"))), [], [])
+//         | Textbox_node(_, _, _) ->
+//             (b, X(R(String_value("textbox"))), [], [])
+//         | Button_node(_, _, _) ->
+//             (b, X(R(String_value("button"))), [], [])
+//         | Inl_script_node(_, _, _) ->
+//             (b, X(R(String_value("inl_script"))), [], [])
+//         | Rem_script_node(_, _, _) ->
+//             (b, X(R(String_value("rem_script"))), [], [])
+//         | Div_node(_, _) ->
+//             (b, X(R(String_value("div"))), [], [])
+//         end
+
+//     | Get_node_contents(X(R(Node_value(dr)))) ->
+//         begin match node_assoc_valid dr b with
+//         | Para_node(_, txt) ->
+//             (b, X(R(String_value(txt))), [], [])
+//         | Link_node(_, _, txt) ->
+//             (b, X(R(String_value(txt))), [], [])
+//         | Button_node(_, txt, _) ->
+//             (b, X(R(String_value(txt))), [], [])
+//         | Inl_script_node(_, e, _) ->
+//             (b, X(R(Code_value(e))), [], [])
+//         | _ ->
+//             let err = "node has no contents" in
+//             (b, X(R(Error(err))), [], [])
+//         end
+//     | Set_node_contents(X(R(Node_value(dr))), X(R(String_value(s)))) ->
+//         begin match node_assoc_valid dr b with
+//         | Para_node(oeid, _) ->
+//             let b' = node_update dr (Para_node(oeid, s)) b in
+//             (b', X(R(String_value(s))), [], [])
+//         | Link_node(oeid, u, _) ->
+//             let b' = node_update dr (Link_node(oeid, u, s)) b in
+//             (b', X(R(String_value(s))), [], [])
+//         | Button_node(oeid, _, hs) ->
+//             let b' = node_update dr (Button_node(oeid, s, hs)) b in
+//             (b', X(R(String_value(s))), [], [])
+//         | _ ->
+//             let err = "node has no string contents" in
+//             (b, X(R(Error(err))), [], [])
+//         end
+//     | Set_node_contents(X(R(Node_value(dr))), X(R(Code_value(e)))) ->
+//         begin match node_assoc_valid dr b with
+//         | Inl_script_node(oeid, _, flag) ->
+//             let b' = node_update dr (Inl_script_node(oeid, e, flag)) b in
+//             (b', X(R(Code_value(e))), [], [])
+//         | _ ->
+//             let err = "node has no script contents" in
+//             (b, X(R(Error(err))), [], [])
+//         end
+
+//     | Get_node_attr(X(R(Node_value(dr))), X(R(String_value("id")))) ->
+//         begin match node_assoc_valid dr b with
+//         | Para_node(Some({ elt_id_value = id }), _)
+//         | Link_node(Some({ elt_id_value = id }), _, _)
+//         | Textbox_node(Some({ elt_id_value = id }), _, _)
+//         | Button_node(Some({ elt_id_value = id }), _, _)
+//         | Inl_script_node(Some({ elt_id_value = id }), _, _)
+//         | Rem_script_node(Some({ elt_id_value = id }), _, _)
+//         | Div_node(Some({ elt_id_value = id }), _) ->
+//             (b, X(R(String_value(id))), [], [])
+//         | _ ->
+//             (b, X(R(Null_value)), [], [])
+//         end
+//     | Set_node_attr(
+//           X(R(Node_value(dr))),
+//           X(R(String_value("id"))),
+//           X(R(Null_value))) ->
+//         begin match node_assoc_valid dr b with
+//         | Para_node(_, text) ->
+//             let b' = node_update dr (Para_node(None, text)) b in
+//             (b', X(R(Null_value)), [], [])
+//         | Link_node(_, u, text) ->
+//             let b' = node_update dr (Link_node(None, u, text)) b in
+//             (b', X(R(Null_value)), [], [])
+//         | Textbox_node(_, s, hs) ->
+//             let b' = node_update dr (Textbox_node(None, s, hs)) b in
+//             (b', X(R(Null_value)), [], [])
+//         | Button_node(_, s, hs) ->
+//             let b' = node_update dr (Button_node(None, s, hs)) b in
+//             (b', X(R(Null_value)), [], [])
+//         | Inl_script_node(_, e, flag) ->
+//             let b' = node_update dr (Inl_script_node(None, e, flag)) b in
+//             (b', X(R(Null_value)), [], [])
+//         | Rem_script_node(_, u, flag) ->
+//             let b' = node_update dr (Rem_script_node(None, u, flag)) b in
+//             (b', X(R(Null_value)), [], [])
+//         | Div_node(_, ns) ->
+//             let b' = node_update dr (Div_node(None, ns)) b in
+//             (b', X(R(Null_value)), [], [])
+//         end
+//     | Set_node_attr(
+//           X(R(Node_value(dr))),
+//           X(R(String_value("id"))),
+//           X(R(String_value(s)))) ->
+//         let oeid = Some({ elt_id_value = s }) in
+//         begin match node_assoc_valid dr b with
+//         | Para_node(_, text) ->
+//             let b' = node_update dr (Para_node(oeid, text)) b in
+//             (b', X(R(Null_value)), [], [])
+//         | Link_node(_, u, text) ->
+//             let b' = node_update dr (Link_node(oeid, u, text)) b in
+//             (b', X(R(Null_value)), [], [])
+//         | Textbox_node(_, s, hs) ->
+//             let b' = node_update dr (Textbox_node(oeid, s, hs)) b in
+//             (b', X(R(Null_value)), [], [])
+//         | Button_node(_, s, hs) ->
+//             let b' = node_update dr (Button_node(oeid, s, hs)) b in
+//             (b', X(R(Null_value)), [], [])
+//         | Inl_script_node(_, e, flag) ->
+//             let b' = node_update dr (Inl_script_node(oeid, e, flag)) b in
+//             (b', X(R(Null_value)), [], [])
+//         | Rem_script_node(_, u, flag) ->
+//             let b' = node_update dr (Rem_script_node(oeid, u, flag)) b in
+//             (b', X(R(Null_value)), [], [])
+//         | Div_node(_, ns) ->
+//             let b' = node_update dr (Div_node(oeid, ns)) b in
+//             (b', X(R(Null_value)), [], [])
+//         end
+
+//     | Get_node_attr(X(R(Node_value(dr))), X(R(String_value("href")))) ->
+//         begin match node_assoc_valid dr b with
+//         | Link_node(_, u, _) ->
+//             (b, X(R(Url_value(u))), [], [])
+//         | _ ->
+//             let err = "node has no 'href' attribute" in
+//             (b, X(R(Error(err))), [], [])
+//         end
+//     | Set_node_attr(
+//           X(R(Node_value(dr))),
+//           X(R(String_value("href"))),
+//           X(R(Url_value(u)))) ->
+//         begin match node_assoc_valid dr b with
+//         | Link_node(oeid, _, text) ->
+//             let b' = node_update dr (Link_node(oeid, u, text)) b in
+//             let oes =
+//               begin match node_page dr b' with
+//               | None -> []
+//               | Some(pr) -> [ page_update_event pr b' ]
+//               end
+//             in
+//             (b', X(R(Url_value(u))), oes, [])
+//         | _ ->
+//             let err = "node has no 'href' attribute" in
+//             (b, X(R(Error(err))), [], [])
+//         end
+
+//     | Get_node_attr(X(R(Node_value(dr))), X(R(String_value("value")))) ->
+//         begin match node_assoc_valid dr b with
+//         | Textbox_node(_, s, _) ->                             
+//             (b, X(R(String_value(s))), [], [])
+//         | _ ->
+//             let err = "node has no 'value' attribute" in
+//             (b, X(R(Error(err))), [], [])
+//         end
+//     | Set_node_attr(
+//           X(R(Node_value(dr))),
+//           X(R(String_value("value"))),
+//           X(R(String_value(s)))) ->
+//         begin match node_assoc_valid dr b with
+//         | Textbox_node(oeid, _, handlers) ->
+//             let b' = node_update dr (Textbox_node(oeid, s, handlers)) b in
+//             let oes =
+//               begin match node_page dr b' with
+//               | None -> []
+//               | Some(pr) -> [ page_update_event pr b' ]
+//               end
+//             in
+//             (b', X(R(String_value(s))), oes, [])
+//         | _ ->
+//             let err = "node has no 'value' attribute" in
+//             (b, X(R(Error(err))), [], [])
+//         end
+
+//     | Get_node_attr(X(R(Node_value(dr))), X(R(String_value("src")))) ->
+//         begin match node_assoc_valid dr b with
+//         | Rem_script_node(_, u, _) ->
+//             (b, X(R(Url_value(u))), [], [])
+//         | _ ->
+//             let err = "node has no 'src' attribute" in
+//             (b, X(R(Error(err))), [], [])
+//         end
+//     | Set_node_attr(
+//           X(R(Node_value(dr))),
+//           X(R(String_value("src"))),
+//           X(R(Url_value(u)))) ->
+//         begin match node_assoc_valid dr b with
+//         | Rem_script_node(oeid, _, flag) ->
+//             let b' = node_update dr (Rem_script_node(oeid, u, flag)) b in
+//             (b', X(R(Url_value(u))), [], [])
+//         | _ ->
+//             let err = "node has no 'src' attribute" in
+//             (b, X(R(Error(err))), [], [])
+//         end
+
+//     | Remove_handlers(X(R(Node_value(dr)))) ->
+//         begin match node_assoc_valid dr b with
+//         | Textbox_node(id, s, _) ->
+//             let dn' = Textbox_node(id, s, []) in
+//             let b' = node_update dr dn' b in
+//             (b', X(R(Null_value)), [], [])
+//         | Button_node(id, s, _) ->
+//             let dn' = Button_node(id, s, []) in
+//             let b' = node_update dr dn' b in
+//             (b', X(R(Null_value)), [], [])
+//         | _ ->
+//             let err = "expected textbox or button node" in
+//             (b, X(R(Error(err))), [], [])
+//         end
+//     | Add_handler(X(R(Node_value(dr))), X(R(Closure(_, _, _, _)))) ->
+//         begin match node_assoc_valid dr b with
+//         | Textbox_node(oeid, str, hs) ->
+//             let b' = node_update dr (Textbox_node(oeid, str, Closure(_, _, _, _) :: hs)) b in
+//             (b', X(R(Null_value)), [], [])
+//         | Button_node(oeid, str, hs) ->
+//             let b' = node_update dr (Button_node(oeid, str, Closure(_, _, _, _) :: hs)) b in
+//             (b', X(R(Null_value)), [], [])
+//         | _ ->
+//             let err = "expected textbox or button node" in
+//             (b, X(R(Error(err))), [], [])
+//         end
+
+//     | Get_parent(X(R(Node_value(dr)))) ->
+//         begin match node_parent dr b with
+//         | Parent_node(parent) ->
+//             (b, X(R(Node_value(parent))), [], [])
+//         | _ ->
+//             (b, X(R(Null_value)), [], [])
+//         end
+//     | Get_child(X(R(Node_value(dr))), X(R(Int_value(i)))) ->
+//         begin match node_assoc_valid dr b with
+//         | Div_node(_, drs) ->
+//             begin if List.length drs <= i then
+//               (b, X(R(Null_value)), [], [])
+//             else
+//               (b, X(R(Node_value(List.nth drs i))), [], [])
+//             end
+//         | _ ->
+//             let err = "expected div node" in
+//             (b, X(R(Error(err))), [], [])
+//         end
+//     | Insert_node(
+//           X(R(Node_value(dr1))),
+//           X(R(Node_value(dr2))),
+//           X(R(Int_value(k)))) ->
+//         begin try
+//           let (b', oes, ts) = node_insert dr1 dr2 k b in
+//           (b', X(R(Null_value)), oes, ts)
+//         with
+//         | Failure("node_insert") ->
+//             let err = "parent node not a div node or a descendant of child" in
+//             (b, X(R(Error(err))), [], [])
+//         | Failure("insert_in_list") ->
+//             (b, X(R(Error("div node has too few children"))), [], [])
+//         end
+//     | Remove_node(X(R(Node_value(dr)))) ->
+//         let (b', oes) = node_remove dr b in
+//         (b', X(R(Null_value)), oes, [])
+
+//     (* congurence rules: evaluation in subexpressions *)
+
+//     | Eval(e1) ->
+//         let (b', e1', oes, ts) = step b e1 in
+//         (b, Eval(e1'), oes, ts)
+//     | Apply(X(R(_)), e2) ->
+//         let (b', e2', oes, ts) = step b e2 in
+//         (b', Apply(X(R(_)), e2'), oes, ts)
+//     | Apply(e1, e2) ->
+//         let (b', e1', oes, ts) = step b e1 in
+//         (b', Apply(e1', e2), oes, ts)
+//     | Prim1(prim, e1) ->
+//         let (b', e1', oes, ts) = step b e1 in
+//         (b', Prim1(prim, e1'), oes, ts)
+//     | Prim2(prim, X(R(_)), e2) ->
+//         let (b', e2', oes, ts) = step b e2 in
+//         (b', Prim2(prim, X(R(_)), e2'), oes, ts)
+//     | Prim2(prim, e1, e2) ->
+//         let (b', e1', oes, ts) = step b e1 in
+//         (b', Prim2(prim, e1', e2), oes, ts)
+//     | Alert(e1) ->
+//         let (b', e1', oes, ts) = step b e1 in
+//         (b', Alert(e1'), oes, ts)
+//     | If(e1, e2, e3) ->
+//         let (b', e1', oes, ts) = step b e1 in
+//         (b', If(e1', e2, e3), oes, ts)
+//     | Set_var(x, e1) ->
+//         let (b', e1', oes, ts) = step b e1 in
+//         (b', Set_var(x, e1'), oes, ts)
+//     | Seq(e1, e2) ->
+//         let (b', e1', oes, ts) = step b e1 in
+//         (b', Seq(e1', e2), oes, ts)
+//     | Get_cookie(X(R(_)), e2) ->
+//         let (b', e2', oes, ts) = step b e2 in
+//         (b', Get_cookie(X(R(_)), e2'), oes, ts)
+//     | Get_cookie(e1, e2) ->
+//         let (b', e1', oes, ts) = step b e1 in
+//         (b', Get_cookie(e1', e2), oes, ts)
+//     | Set_cookie((X(R(_))), (X(R(_))), e3) ->
+//         let (b', e3', oes, ts) = step b e3 in
+//         (b', Set_cookie(X(R(_)), X(R(_)), e3'), oes, ts)
+//     | Set_cookie((X(R(_))), e2, e3) ->
+//         let (b', e2', oes, ts) = step b e2 in
+//         (b', Set_cookie(X(R(_)), e2', e3), oes, ts)
+//     | Set_cookie(e1, e2, e3) ->
+//         let (b', e1', oes, ts) = step b e1 in
+//         (b', Set_cookie(e1', e2, e3), oes, ts)
+//     | Xhr((X(R(_))), (X(R(_))), e3) ->
+//         let (b', e3', oes, ts) = step b e3 in
+//         (b', Xhr(X(R(_)), X(R(_)), e3'), oes, ts)
+//     | Xhr((X(R(_))), e2, e3) ->
+//         let (b', e2', oes, ts) = step b e2 in
+//         (b', Xhr(X(R(_)), e2', e3), oes, ts)
+//     | Xhr(e1, e2, e3) ->
+//         let (b', e1', oes, ts) = step b e1 in
+//         (b', Xhr(e1', e2, e3), oes, ts)
+//     | Named_win(e1) ->
+//         let (b', e1', oes, ts) = step b e1 in
+//         (b', Named_win(e1'), oes, ts)
+//     | Open_win(e1) ->
+//         let (b', e1', oes, ts) = step b e1 in
+//         (b', Open_win(e1'), oes, ts)
+//     | Open_named_win(X(R(_)), e2) ->
+//         let (b', e2', oes, ts) = step b e2 in
+//         (b', Open_named_win(X(R(_)), e2'), oes, ts)
+//     | Open_named_win(e1, e2) ->
+//         let (b', e1', oes, ts) = step b e1 in
+//         (b', Open_named_win(e1', e2), oes, ts)
+//     | Close_win(e1) ->
+//         let (b', e1', oes, ts) = step b e1 in
+//         (b', Close_win(e1'), oes, ts)
+//     | Navigate_win(X(R(_)), e2) ->
+//         let (b', e2', oes, ts) = step b e2 in
+//         (b', Navigate_win(X(R(_)), e2'), oes, ts)
+//     | Navigate_win(e1, e2) ->
+//         let (b', e1', oes, ts) = step b e1 in
+//         (b', Navigate_win(e1', e2), oes, ts)
+//     | Is_win_closed(e1) ->
+//         let (b', e1', oes, ts) = step b e1 in
+//         (b', Is_win_closed(e1'), oes, ts)
+//     | Get_win_opener(e1) ->
+//         let (b', e1', oes, ts) = step b e1 in
+//         (b', Get_win_opener(e1'), oes, ts)
+//     | Get_win_location(e1) ->
+//         let (b', e1', oes, ts) = step b e1 in
+//         (b', Get_win_location(e1'), oes, ts)
+//     | Get_win_name(e1) ->
+//         let (b', e1', oes, ts) = step b e1 in
+//         (b', Get_win_name(e1'), oes, ts)
+//     | Set_win_name(X(R(_)), e2) ->
+//         let (b', e2', oes, ts) = step b e2 in
+//         (b', Set_win_name(X(R(_)), e2'), oes, ts)
+//     | Set_win_name(e1, e2) ->
+//         let (b', e1', oes, ts) = step b e1 in
+//         (b', Set_win_name(e1', e2), oes, ts)
+//     | Get_win_root_node(e1) ->
+//         let (b', e1', oes, ts) = step b e1 in
+//         (b', Get_win_root_node(e1'), oes, ts)
+//     | Set_win_root_node(X(R(_)), e2) ->
+//         let (b', e2', oes, ts) = step b e2 in
+//         (b', Set_win_root_node(X(R(_)), e2'), oes, ts)
+//     | Set_win_root_node(e1, e2) ->
+//         let (b', e1', oes, ts) = step b e1 in
+//         (b', Set_win_root_node(e1', e2), oes, ts)
+//     | Get_win_var(e1, x) ->
+//         let (b', e1', oes, ts) = step b e1 in
+//         (b', Get_win_var(e1', x), oes, ts)
+//     | Set_win_var(X(R(_)), x, e2) ->
+//         let (b', e2', oes, ts) = step b e2 in
+//         (b', Set_win_var(X(R(_)), x, e2'), oes, ts)
+//     | Set_win_var(e1, x, e2) ->
+//         let (b', e1', oes, ts) = step b e1 in
+//         (b', Set_win_var(e1', x, e2), oes, ts)
+//     | New_node(e1) ->
+//         let (b', e1', oes, ts) = step b e1 in
+//         (b', New_node(e1'), oes, ts)
+//     | Get_node_type(e1) ->
+//         let (b', e1', oes, ts) = step b e1 in
+//         (b', Get_node_type(e1'), oes, ts)
+//     | Get_node_contents(e1) -> 
+//        let (b', e1', oes, ts) = step b e1 in
+//         (b', Get_node_contents(e1'), oes, ts)
+//     | Set_node_contents(X(R(_)), e2) ->
+//         let (b', e2', oes, ts) = step b e2 in
+//         (b', Set_node_contents(X(R(_)), e2'), oes, ts)
+//     | Set_node_contents(e1, e2) ->
+//         let (b', e1', oes, ts) = step b e1 in
+//         (b', Set_node_contents(e1', e2), oes, ts)
+//     | Get_node_attr(X(R(_)), e2) ->
+//         let (b', e2', oes, ts) = step b e2 in
+//         (b', Get_node_attr(X(R(_)), e2'), oes, ts)
+//     | Get_node_attr(e1, e2) ->
+//         let (b', e1', oes, ts) = step b e1 in
+//         (b', Get_node_attr(e1', e2), oes, ts)
+//     | Set_node_attr((X(R(_))), (X(R(_))), e3) ->
+//         let (b', e3', oes, ts) = step b e3 in
+//         (b', Set_node_attr(X(R(_)), X(R(_)), e3'), oes, ts)
+//     | Set_node_attr((X(R(_))), e2, e3) ->
+//         let (b', e2', oes, ts) = step b e2 in
+//         (b', Set_node_attr(X(R(_)), e2', e3), oes, ts)
+//     | Set_node_attr(e1, e2, e3) ->
+//         let (b', e1', oes, ts) = step b e1 in
+//         (b', Set_node_attr(e1', e2, e3), oes, ts)
+//     | Remove_handlers(e1) ->
+//         let (b', e1', oes, ts) = step b e1 in
+//         (b', Remove_handlers(e1'), oes, ts)
+//     | Add_handler((X(R(_))), e2) ->
+//         let (b', e2', oes, ts) = step b e2 in
+//         (b', Add_handler(X(R(_)), e2'), oes, ts)
+//     | Add_handler(e1, e2) ->
+//         let (b', e1', oes, ts) = step b e1 in
+//         (b', Add_handler(e1', e2), oes, ts)
+//     | Get_child(X(R(_)), e2) ->
+//         let (b', e2', oes, ts) = step b e2 in
+//         (b', Get_child(X(R(_)), e2'), oes, ts)
+//     | Get_parent(e1) ->
+//         let (b', e1', oes, ts) = step b e1 in
+//         (b', Get_parent(e1'), oes, ts)
+//     | Get_child(e1, e2) ->
+//         let (b', e1', oes, ts) = step b e1 in
+//         (b', Get_child(e1', e2), oes, ts)
+//     | Insert_node((X(R(_))), (X(R(_))), e3) ->
+//         let (b', e3', oes, ts) = step b e3 in
+//         (b', Insert_node(X(R(_)), X(R(_)), e3'), oes, ts)
+//     | Insert_node((X(R(_))), e2, e3) ->
+//         let (b', e2', oes, ts) = step b e2 in
+//         (b', Insert_node(X(R(_)), e2', e3), oes, ts)
+//     | Insert_node(e1, e2, e3) ->
+//         let (b', e1', oes, ts) = step b e1 in
+//         (b', Insert_node(e1', e2, e3), oes, ts)
+//     | Remove_node(e1) ->
+//         let (b', e1', oes, ts) = step b e1 in
+//         (b', Remove_node(e1'), oes, ts)
+
+//     end
